cheririscV/CapGlobalenvs.v
@@ -1,0 +1,2529 @@
+(* *********************************************************************)
+(*                                                                     *)
+(*              The Compcert verified compiler                         *)
+(*                                                                     *)
+(*          Xavier Leroy, INRIA Paris-Rocquencourt                     *)
+(*                                                                     *)
+(*  Copyright Institut National de Recherche en Informatique et en     *)
+(*  Automatique.  All rights reserved.  This file is distributed       *)
+(*  under the terms of the GNU General Public License as published by  *)
+(*  the Free Software Foundation, either version 2 of the License, or  *)
+(*  (at your option) any later version.  This file is also distributed *)
+(*  under the terms of the INRIA Non-Commercial License Agreement.     *)
+(*                                                                     *)
+(* *********************************************************************)
+
+(** Global environments are a component of the dynamic semantics of
+  all languages involved in the compiler.  A global environment
+  maps symbol names (names of functions and of global variables)
+  to the corresponding memory addresses.  It also maps memory addresses
+  of functions to the corresponding function descriptions.
+
+  Global environments, along with the initial memory state at the beginning
+  of program execution, are built from the program of interest, as follows:
+- A distinct memory address is assigned to each function of the program.
+  These function addresses use negative numbers to distinguish them from
+  addresses of memory blocks.  The associations of function name to function
+  address and function address to function description are recorded in
+  the global environment.
+- For each global variable, a memory block is allocated and associated to
+  the name of the variable.
+
+  These operations reflect (at a high level of abstraction) what takes
+  place during program linking and program loading in a real operating
+  system. *)
+
+(** This file consists of the altered definition of globalenvs for the
+capability machine backend, where symbols are now matched to capabilities *)
+
+Require Import Recdef.
+Require Import Zwf.
+Require Import Axioms Coqlib Errors Maps CapAST Linking.
+Require Import Integers Floats OCapValues CapMemory.
+
+Notation "s #1" := (fst s) (at level 9, format "s '#1'") : pair_scope.
+Notation "s #2" := (snd s) (at level 9, format "s '#2'") : pair_scope.
+
+Local Open Scope pair_scope.
+Local Open Scope error_monad_scope.
+
+Set Implicit Arguments.
+
+(** Auxiliary function for initialization of global variables. *)
+
+(** The following version assumes an init capability *)
+Function store_zeros (m: mem) (ptr: occap) (n: Z) (cp: compartment) {wf (Zwf 0) n}: occap * mem + error_kind :=
+  if zle n 0 then inl (ptr,m) else
+    match Mem.store DIR CMint8unsigned m ptr 0 OCVzero cp, incr_addr_stk ptr 1 with
+    | inl (_,m'),Some ptr' => store_zeros m' ptr' (n - 1) cp
+    | inr err,_ => inr err
+    | inl _, None => inr CapErr
+    end.
+Proof.
+  intros. red. omega.
+  apply Zwf_well_founded.
+Qed.
+
+(* To avoid useless definitions of inductors in extracted code. *)
+Local Unset Elimination Schemes.
+Local Unset Case Analysis Schemes.
+
+(** * Symbol environments *)
+
+(** Symbol environments are a restricted view of global environments,
+  focusing on symbol names and their associated blocks.  They do not
+  contain mappings from blocks to function or variable definitions. *)
+
+Module Senv.
+
+Record t: Type := mksenv {
+  (** Operations *)
+  find_symbol: ident -> option occap;
+  public_symbol: ident -> bool;
+  invert_symbol: occap -> option ident;
+  block_is_volatile: occap -> bool;
+  (** Properties *)
+  find_symbol_injective:
+    forall id1 id2 b, find_symbol id1 = Some b -> find_symbol id2 = Some b -> id1 = id2;
+  invert_find_symbol:
+    forall id b, invert_symbol b = Some id -> find_symbol id = Some b;
+  find_invert_symbol:
+    forall id b, find_symbol id = Some b -> invert_symbol b = Some id;
+  public_symbol_exists:
+    forall id, public_symbol id = true -> exists b, find_symbol id = Some b;
+}.
+
+Definition symbol_address (ge: t) (id: ident) (ofs: ptrofs) : ocval :=
+  match find_symbol ge id with
+  | Some c => OCVcap c
+  | None => OCVundef
+  end.
+
+(* Theorem shift_symbol_address: *)
+(*   forall ge id ofs delta, *)
+(*   symbol_address ge id (Ptrofs.add ofs delta) = Val.offset_ptr (symbol_address ge id ofs) delta. *)
+(* Proof. *)
+(*   intros. unfold symbol_address, Val.offset_ptr. destruct (find_symbol ge id); auto. *)
+(* Qed. *)
+
+(* Theorem shift_symbol_address_32: *)
+(*   forall ge id ofs n, *)
+(*   Archi.ptr64 = false -> *)
+(*   symbol_address ge id (Ptrofs.add ofs (Ptrofs.of_int n)) = Val.add (symbol_address ge id ofs) (Vint n). *)
+(* Proof. *)
+(*   intros. unfold symbol_address. destruct (find_symbol ge id). *)
+(* - unfold Val.add. rewrite H. auto. *)
+(* - auto. *)
+(* Qed. *)
+
+(* Theorem shift_symbol_address_64: *)
+(*   forall ge id ofs n, *)
+(*   Archi.ptr64 = true -> *)
+(*   symbol_address ge id (Ptrofs.add ofs (Ptrofs.of_int64 n)) = Val.addl (symbol_address ge id ofs) (Vlong n). *)
+(* Proof. *)
+(*   intros. unfold symbol_address. destruct (find_symbol ge id). *)
+(* - unfold Val.addl. rewrite H. auto. *)
+(* - auto. *)
+(* Qed. *)
+
+Definition equiv (se1 se2: t) : Prop :=
+     (forall id, find_symbol se2 id = find_symbol se1 id)
+  /\ (forall id, public_symbol se2 id = public_symbol se1 id)
+  /\ (forall b, block_is_volatile se2 b = block_is_volatile se1 b).
+
+End Senv.
+
+Module Genv.
+
+(** * Global environments *)
+
+Section GENV.
+
+Variable F: Type.  (**r The type of function descriptions *)
+Variable V: Type.  (**r The type of information attached to variables *) 
+
+Variable globdef_size: (globdef F V) -> nat.
+
+Context {CF: has_comp F}.
+
+(** The type of global environments. *)
+
+Definition cap_to_pos_lo (ptr: occap) : positive :=
+  Z.to_pos (Ptrofs.unsigned (get_lo ptr)).
+
+Record t: Type := mkgenv {
+  genv_public: list ident;              (**r which symbol names are public *)
+  genv_symb: PTree.t occap;             (**r mapping symbol -> capability *)
+  genv_defs: PTree.t (globdef F V);     (**r mapping the lower bound of cap -> definition *)
+  genv_next: ptrofs;                     (**r next symbol pointer *)
+  genv_policy: Policy.t;                (**r policy *)
+  genv_symb_range: forall id c, PTree.get id genv_symb = Some c -> Ptrofs.lt (get_lo c) genv_next = true;
+  genv_defs_range: forall ptr g, PTree.get (cap_to_pos_lo ptr) genv_defs = Some g -> Ptrofs.lt (get_lo ptr) genv_next = true;
+  genv_vars_inj: forall id1 id2 b,
+    PTree.get id1 genv_symb = Some b -> PTree.get id2 genv_symb = Some b -> id1 = id2
+}.
+
+(** ** Lookup functions *)
+
+(** [find_symbol ge id] returns the block associated with the given name, if any *)
+
+Definition find_symbol (ge: t) (id: ident) : option occap :=
+  PTree.get id ge.(genv_symb).
+
+(** [symbol_address ge id ofs] returns a pointer into the block associated
+  with [id], at byte offset [ofs].  [Vundef] is returned if no block is associated
+  to [id]. *)
+
+Definition symbol_address (ge: t) (id: ident) (ofs: ptrofs) : ocval :=
+  match find_symbol ge id with
+  | Some c => OCVcap c
+  | None => OCVundef
+  end.
+
+(** [public_symbol ge id] says whether the name [id] is public and defined. *)
+
+Definition public_symbol (ge: t) (id: ident) : bool :=
+  match find_symbol ge id with
+  | None => false
+  | Some _ => In_dec ident_eq id ge.(genv_public)
+  end.
+
+(** [find_def ge b] returns the global definition associated with the given capability. *)
+
+Definition find_def (ge: t) (ptr: occap) : option (globdef F V) :=
+  PTree.get (cap_to_pos_lo ptr) ge.(genv_defs).
+
+(** [find_funct_ptr ge b] returns the function description associated with
+    the given address. *)
+
+Definition find_funct_ptr (ge: t) (ptr: occap) : option F :=
+  match find_def ge ptr with Some (Gfun f) => Some f | _ => None end.
+
+Definition find_funct_size (ge: t) (lo: positive) : nat :=
+  match  PTree.get lo ge.(genv_defs) with Some f => globdef_size f | None => 0 end.
+  
+(** [find_funct] is similar to [find_funct_ptr], but the function
+    address is given as a value, which must be a memory capability
+    with address pointing to the base. *)
+
+Definition find_funct (ge: t) (v: ocval) : option F :=
+  match v with
+  | OCVcap c =>
+      if Ptrofs.eq_dec (get_lo c) (get_addr c) &&
+      then find_funct_ptr ge c
+      else None
+  | _ => None
+  end.
+
+(** [find_comp ge v] finds the compartment associated with the pointer [v] as it
+    is recorded in [ge]. *)
+
+Definition find_comp (ge: t) (v: val) : compartment :=
+  match v with
+  | Vptr b _ =>
+    match find_funct_ptr ge b with
+    | Some f => (comp_of f)
+    | None   => default_compartment
+    end
+  | _ => default_compartment
+  end.
+
+Lemma find_comp_null:
+  forall ge, find_comp ge Vnullptr = default_compartment.
+Proof.
+  unfold find_comp, Vnullptr.
+  now destruct Archi.ptr64.
+Qed.
+
+(** [invert_symbol ge b] returns the name associated with the given block, if any *)
+
+Definition invert_symbol (ge: t) (b: block) : option ident :=
+  PTree.fold
+    (fun res id b' => if eq_block b b' then Some id else res)
+    ge.(genv_symb) None.
+
+(** [find_var_info ge b] returns the information attached to the variable
+   at address [b]. *)
+
+Definition find_var_info (ge: t) (b: block) : option (globvar V) :=
+  match find_def ge b with Some (Gvar v) => Some v | _ => None end.
+
+(** [block_is_volatile ge b] returns [true] if [b] points to a global variable
+  of volatile type, [false] otherwise. *)
+
+Definition block_is_volatile (ge: t) (b: block) : bool :=
+  match find_var_info ge b with
+  | None => false
+  | Some gv => gv.(gvar_volatile)
+  end.
+
+(** ** Constructing the global environment *)
+
+Program Definition add_global (ge: t) (idg: ident * globdef F V) : t :=
+  @mkgenv
+    ge.(genv_public)
+    (PTree.set idg#1 ge.(genv_next) ge.(genv_symb))
+    (PTree.set ge.(genv_next) idg#2 ge.(genv_defs))
+    (Pos.succ ge.(genv_next))
+    (genv_policy ge)
+    _ _ _.
+Next Obligation.
+  destruct ge; simpl in *.
+  rewrite PTree.gsspec in H. destruct (peq id i). inv H. apply Plt_succ.
+  apply Plt_trans_succ; eauto.
+Qed.
+Next Obligation.
+  destruct ge; simpl in *.
+  rewrite PTree.gsspec in H. destruct (peq b genv_next0).
+  inv H. apply Plt_succ.
+  apply Plt_trans_succ; eauto.
+Qed.
+Next Obligation.
+  destruct ge; simpl in *.
+  rewrite PTree.gsspec in H. rewrite PTree.gsspec in H0.
+  destruct (peq id1 i); destruct (peq id2 i).
+  congruence.
+  inv H. eelim Plt_strict. eapply genv_symb_range0; eauto.
+  inv H0. eelim Plt_strict. eapply genv_symb_range0; eauto.
+  eauto.
+Qed.
+
+Definition add_globals (ge: t) (gl: list (ident * globdef F V)) : t :=
+  List.fold_left add_global gl ge.
+
+Lemma add_globals_app:
+  forall gl2 gl1 ge,
+  add_globals ge (gl1 ++ gl2) = add_globals (add_globals ge gl1) gl2.
+Proof.
+  intros. apply fold_left_app.
+Qed.
+
+Program Definition empty_genv (pub: list ident) (pol: Policy.t): t :=
+  @mkgenv pub (PTree.empty _) (PTree.empty _) 1%positive pol _ _ _.
+Next Obligation.
+  rewrite PTree.gempty in H. discriminate.
+Qed.
+Next Obligation.
+  rewrite PTree.gempty in H. discriminate.
+Qed.
+Next Obligation.
+  rewrite PTree.gempty in H. discriminate.
+Qed.
+
+Definition globalenv (p: program F V) :=
+  add_globals (empty_genv p.(prog_public) p.(prog_pol)) p.(prog_defs).
+
+(** Proof principles *)
+
+Section GLOBALENV_PRINCIPLES.
+
+Variable P: t -> Prop.
+
+Lemma add_globals_preserves:
+  forall gl ge,
+  (forall ge id g, P ge -> In (id, g) gl -> P (add_global ge (id, g))) ->
+  P ge -> P (add_globals ge gl).
+Proof.
+  induction gl; simpl; intros.
+  auto.
+  destruct a. apply IHgl; auto.
+Qed.
+
+Lemma add_globals_ensures:
+  forall id g gl ge,
+  (forall ge id g, P ge -> In (id, g) gl -> P (add_global ge (id, g))) ->
+  (forall ge, P (add_global ge (id, g))) ->
+  In (id, g) gl -> P (add_globals ge gl).
+Proof.
+  induction gl; simpl; intros.
+  contradiction.
+  destruct H1. subst a. apply add_globals_preserves; auto.
+  apply IHgl; auto.
+Qed.
+
+Lemma add_globals_unique_preserves:
+  forall id gl ge,
+  (forall ge id1 g, P ge -> In (id1, g) gl -> id1 <> id -> P (add_global ge (id1, g))) ->
+  ~In id (map fst gl) -> P ge -> P (add_globals ge gl).
+Proof.
+  induction gl; simpl; intros.
+  auto.
+  destruct a. apply IHgl; auto.
+Qed.
+
+Lemma add_globals_unique_ensures:
+  forall gl1 id g gl2 ge,
+  (forall ge id1 g1, P ge -> In (id1, g1) gl2 -> id1 <> id -> P (add_global ge (id1, g1))) ->
+  (forall ge, P (add_global ge (id, g))) ->
+  ~In id (map fst gl2) -> P (add_globals ge (gl1 ++ (id, g) :: gl2)).
+Proof.
+  intros. rewrite add_globals_app. simpl. apply add_globals_unique_preserves with id; auto.
+Qed.
+
+Remark in_norepet_unique:
+  forall id g (gl: list (ident * globdef F V)),
+  In (id, g) gl -> list_norepet (map fst gl) ->
+  exists gl1 gl2, gl = gl1 ++ (id, g) :: gl2 /\ ~In id (map fst gl2).
+Proof.
+  induction gl as [|[id1 g1] gl]; simpl; intros.
+  contradiction.
+  inv H0. destruct H.
+  inv H. exists nil, gl. auto.
+  exploit IHgl; eauto. intros (gl1 & gl2 & X & Y).
+  exists ((id1, g1) :: gl1), gl2; split; auto. rewrite X; auto.
+Qed.
+
+Lemma add_globals_norepet_ensures:
+  forall id g gl ge,
+  (forall ge id1 g1, P ge -> In (id1, g1) gl -> id1 <> id -> P (add_global ge (id1, g1))) ->
+  (forall ge, P (add_global ge (id, g))) ->
+  In (id, g) gl -> list_norepet (map fst gl) -> P (add_globals ge gl).
+Proof.
+  intros. exploit in_norepet_unique; eauto. intros (gl1 & gl2 & X & Y).
+  subst gl. apply add_globals_unique_ensures; auto. intros. eapply H; eauto.
+  apply in_or_app; simpl; auto.
+Qed.
+
+End GLOBALENV_PRINCIPLES.
+
+(** ** Properties of the operations over global environments *)
+
+Theorem public_symbol_exists:
+  forall ge id, public_symbol ge id = true -> exists b, find_symbol ge id = Some b.
+Proof.
+  unfold public_symbol; intros. destruct (find_symbol ge id) as [b|].
+  exists b; auto.
+  discriminate.
+Qed.
+
+Theorem shift_symbol_address:
+  forall ge id ofs delta,
+  symbol_address ge id (Ptrofs.add ofs delta) = Val.offset_ptr (symbol_address ge id ofs) delta.
+Proof.
+  intros. unfold symbol_address, Val.offset_ptr. destruct (find_symbol ge id); auto.
+Qed.
+
+Theorem shift_symbol_address_32:
+  forall ge id ofs n,
+  Archi.ptr64 = false ->
+  symbol_address ge id (Ptrofs.add ofs (Ptrofs.of_int n)) = Val.add (symbol_address ge id ofs) (Vint n).
+Proof.
+  intros. unfold symbol_address. destruct (find_symbol ge id).
+- unfold Val.add. rewrite H. auto.
+- auto.
+Qed.
+
+Theorem shift_symbol_address_64:
+  forall ge id ofs n,
+  Archi.ptr64 = true ->
+  symbol_address ge id (Ptrofs.add ofs (Ptrofs.of_int64 n)) = Val.addl (symbol_address ge id ofs) (Vlong n).
+Proof.
+  intros. unfold symbol_address. destruct (find_symbol ge id).
+- unfold Val.addl. rewrite H. auto.
+- auto.
+Qed.
+
+Theorem find_funct_inv:
+  forall ge v f,
+  find_funct ge v = Some f -> exists b, v = Vptr b Ptrofs.zero.
+Proof.
+  intros until f; unfold find_funct.
+  destruct v; try congruence.
+  destruct (Ptrofs.eq_dec i Ptrofs.zero); try congruence.
+  intros. exists b; congruence.
+Qed.
+
+Theorem find_funct_find_funct_ptr:
+  forall ge b,
+  find_funct ge (Vptr b Ptrofs.zero) = find_funct_ptr ge b.
+Proof.
+  intros; simpl. apply dec_eq_true.
+Qed.
+
+Theorem find_funct_ptr_iff:
+  forall ge b f,
+  find_funct_ptr ge b = Some f <->
+  find_def ge b = Some (Gfun f).
+Proof.
+  intros. unfold find_funct_ptr.
+  destruct (find_def ge b) as [[f1|v1]|]; intuition congruence.
+Qed.
+
+Theorem find_var_info_iff:
+  forall ge b v,
+  find_var_info ge b = Some v <->
+  find_def ge b = Some (Gvar v).
+Proof.
+  intros. unfold find_var_info.
+  destruct (find_def ge b) as [[f1|v1]|]; intuition congruence.
+Qed.
+
+Theorem find_def_symbol:
+  forall p id g,
+  (prog_defmap p)!id = Some g <-> exists b, find_symbol (globalenv p) id = Some b /\ find_def (globalenv p) b = Some g.
+Proof.
+  intros.
+  set (P := fun m ge => m!id = Some g <-> exists b, find_symbol ge id = Some b /\ find_def ge b = Some g).
+  assert (REC: forall l m ge,
+            P m ge ->
+            P (fold_left (fun m idg => PTree.set idg#1 idg#2 m) l m)
+              (add_globals ge l)).
+  { induction l as [ | [id1 g1] l]; intros; simpl.
+  - auto.
+  - apply IHl. unfold P, add_global, find_symbol, find_def; simpl.
+    rewrite ! PTree.gsspec. destruct (peq id id1).
+    + subst id1. split; intros.
+      inv H0. exists (genv_next ge); split; auto. apply PTree.gss.
+      destruct H0 as (b & A & B). inv A. rewrite PTree.gss in B. auto.
+    + red in H; rewrite H. split.
+      intros (b & A & B). exists b; split; auto. rewrite PTree.gso; auto.
+      apply Plt_ne. eapply genv_symb_range; eauto.
+      intros (b & A & B). rewrite PTree.gso in B. exists b; auto.
+      apply Plt_ne. eapply genv_symb_range; eauto.
+  }
+  apply REC. unfold P, find_symbol, find_def; simpl.
+  rewrite ! PTree.gempty. split.
+  congruence.
+  intros (b & A & B); congruence.
+Qed.
+
+Theorem find_symbol_exists:
+  forall p id g,
+  In (id, g) (prog_defs p) ->
+  exists b, find_symbol (globalenv p) id = Some b.
+Proof.
+  intros. unfold globalenv. eapply add_globals_ensures; eauto.
+(* preserves *)
+  intros. unfold find_symbol; simpl. rewrite PTree.gsspec. destruct (peq id id0).
+  econstructor; eauto.
+  auto.
+(* ensures *)
+  intros. unfold find_symbol; simpl. rewrite PTree.gss. econstructor; eauto.
+Qed.
+
+Theorem find_symbol_inversion : forall p x b,
+  find_symbol (globalenv p) x = Some b ->
+  In x (prog_defs_names p).
+Proof.
+  intros until b; unfold globalenv. eapply add_globals_preserves.
+(* preserves *)
+  unfold find_symbol; simpl; intros. rewrite PTree.gsspec in H1.
+  destruct (peq x id). subst x. change id with (fst (id, g)). apply List.in_map; auto.
+  auto.
+(* base *)
+  unfold find_symbol; simpl; intros. rewrite PTree.gempty in H. discriminate.
+Qed.
+
+Theorem find_symbol_find_def_inversion : forall p x b,
+  find_symbol (globalenv p) x = Some b ->
+  exists g, find_def (globalenv p) b = Some g.
+Proof.
+  intros until b. unfold globalenv. eapply add_globals_preserves.
+  - unfold find_symbol, find_def, add_global. simpl.
+    intros ge id g IH IN SYMBOL.
+    destruct (Pos.eq_dec id x) as [->|neq].
+    + rewrite PTree.gss in SYMBOL. injection SYMBOL as <-.
+      rewrite PTree.gss. eauto.
+    + rewrite PTree.gso in SYMBOL; eauto.
+      destruct IH as [g' IH]; eauto.
+      pose proof (genv_defs_range _ _ IH) as FRESH.
+      rewrite PTree.gso; eauto.
+      now apply Plt_ne.
+  - unfold find_symbol. simpl. now rewrite PTree.gempty.
+Qed.
+
+Theorem find_def_inversion:
+  forall p b g,
+  find_def (globalenv p) b = Some g ->
+  exists id, In (id, g) (prog_defs p).
+Proof.
+  intros until g. unfold globalenv. apply add_globals_preserves.
+(* preserves *)
+  unfold find_def; simpl; intros.
+  rewrite PTree.gsspec in H1. destruct (peq b (genv_next ge)).
+  inv H1. exists id; auto.
+  auto.
+(* base *)
+  unfold find_def; simpl; intros. rewrite PTree.gempty in H. discriminate.
+Qed.
+
+Corollary find_funct_ptr_inversion:
+  forall p b f,
+  find_funct_ptr (globalenv p) b = Some f ->
+  exists id, In (id, Gfun f) (prog_defs p).
+Proof.
+  intros. apply find_def_inversion with b. apply find_funct_ptr_iff; auto.
+Qed.
+
+Corollary find_funct_inversion:
+  forall p v f,
+  find_funct (globalenv p) v = Some f ->
+  exists id, In (id, Gfun f) (prog_defs p).
+Proof.
+  intros. exploit find_funct_inv; eauto. intros [b EQ]. subst v.
+  rewrite find_funct_find_funct_ptr in H.
+  eapply find_funct_ptr_inversion; eauto.
+Qed.
+
+Theorem find_funct_ptr_prop:
+  forall (P: F -> Prop) p b f,
+  (forall id f, In (id, Gfun f) (prog_defs p) -> P f) ->
+  find_funct_ptr (globalenv p) b = Some f ->
+  P f.
+Proof.
+  intros. exploit find_funct_ptr_inversion; eauto. intros [id IN]. eauto.
+Qed.
+
+Theorem find_funct_prop:
+  forall (P: F -> Prop) p v f,
+  (forall id f, In (id, Gfun f) (prog_defs p) -> P f) ->
+  find_funct (globalenv p) v = Some f ->
+  P f.
+Proof.
+  intros. exploit find_funct_inversion; eauto. intros [id IN]. eauto.
+Qed.
+
+Theorem global_addresses_distinct:
+  forall ge id1 id2 b1 b2,
+  id1 <> id2 ->
+  find_symbol ge id1 = Some b1 ->
+  find_symbol ge id2 = Some b2 ->
+  b1 <> b2.
+Proof.
+  intros. red; intros; subst. elim H. destruct ge. eauto.
+Qed.
+
+Theorem invert_find_symbol:
+  forall ge id b,
+  invert_symbol ge b = Some id -> find_symbol ge id = Some b.
+Proof.
+  intros until b; unfold find_symbol, invert_symbol.
+  apply PTree_Properties.fold_rec.
+  intros. rewrite H in H0; auto.
+  congruence.
+  intros. destruct (eq_block b v). inv H2. apply PTree.gss.
+  rewrite PTree.gsspec. destruct (peq id k).
+  subst. assert (m!k = Some b) by auto. congruence.
+  auto.
+Qed.
+
+Theorem find_invert_symbol:
+  forall ge id b,
+  find_symbol ge id = Some b -> invert_symbol ge b = Some id.
+Proof.
+  intros until b.
+  assert (find_symbol ge id = Some b -> exists id', invert_symbol ge b = Some id').
+  unfold find_symbol, invert_symbol.
+  apply PTree_Properties.fold_rec.
+  intros. rewrite H in H0; auto.
+  rewrite PTree.gempty; congruence.
+  intros. destruct (eq_block b v). exists k; auto.
+  rewrite PTree.gsspec in H2. destruct (peq id k).
+  inv H2. congruence. auto.
+
+  intros; exploit H; eauto. intros [id' A].
+  assert (id = id'). eapply genv_vars_inj; eauto. apply invert_find_symbol; auto.
+  congruence.
+Qed.
+
+Definition advance_next (gl: list (ident * globdef F V)) (x: positive) :=
+  List.fold_left (fun n g => Pos.succ n) gl x.
+
+Remark genv_next_add_globals:
+  forall gl ge,
+  genv_next (add_globals ge gl) = advance_next gl (genv_next ge).
+Proof.
+  induction gl; simpl; intros.
+  auto.
+  rewrite IHgl. auto.
+Qed.
+
+Remark genv_public_add_globals:
+  forall gl ge,
+  genv_public (add_globals ge gl) = genv_public ge.
+Proof.
+  induction gl; simpl; intros.
+  auto.
+  rewrite IHgl; auto.
+Qed.
+
+Remark genv_pol_add_globals:
+  forall gl ge,
+  genv_policy (add_globals ge gl) = genv_policy ge.
+Proof.
+  induction gl; simpl; intros.
+  auto.
+  rewrite IHgl; auto.
+Qed.
+
+Theorem globalenv_public:
+  forall p, genv_public (globalenv p) = prog_public p.
+Proof.
+  unfold globalenv; intros. rewrite genv_public_add_globals. auto.
+Qed.
+
+Theorem block_is_volatile_below:
+  forall ge b, block_is_volatile ge b = true ->  Plt b ge.(genv_next).
+Proof.
+  unfold block_is_volatile; intros. destruct (find_var_info ge b) as [[c gv]|] eqn:FV.
+  rewrite find_var_info_iff in FV. eapply genv_defs_range; eauto.
+  discriminate.
+Qed.
+
+(** ** Coercing a global environment into a symbol environment *)
+
+Definition to_senv (ge: t) : Senv.t :=
+ @Senv.mksenv
+    (find_symbol ge)
+    (public_symbol ge)
+    (invert_symbol ge)
+    (block_is_volatile ge)
+    ge.(genv_next)
+    ge.(genv_vars_inj)
+    (invert_find_symbol ge)
+    (find_invert_symbol ge)
+    (public_symbol_exists ge)
+    ge.(genv_symb_range)
+    (block_is_volatile_below ge).
+
+(** * Construction of the initial memory state *)
+
+Section INITMEM.
+
+Variable ge: t.
+
+Definition store_init_data (m: mem) (b: block) (p: Z) (id: init_data) (cp: compartment) : option mem :=
+  match id with
+  | Init_int8 n => Mem.store Mint8unsigned m b p (Vint n) cp
+  | Init_int16 n => Mem.store Mint16unsigned m b p (Vint n) cp
+  | Init_int32 n => Mem.store Mint32 m b p (Vint n) cp
+  | Init_int64 n => Mem.store Mint64 m b p (Vlong n) cp
+  | Init_float32 n => Mem.store Mfloat32 m b p (Vsingle n) cp
+  | Init_float64 n => Mem.store Mfloat64 m b p (Vfloat n) cp
+  | Init_addrof symb ofs =>
+      match find_symbol ge symb with
+      | None => None
+      | Some b' => Mem.store Mptr m b p (Vptr b' ofs) cp
+      end
+  | Init_space n => Some m
+  end.
+
+Fixpoint store_init_data_list (m: mem) (b: block) (p: Z) (idl: list init_data)
+                              (cp : compartment)
+                              {struct idl}: option mem :=
+  match idl with
+  | nil => Some m
+  | id :: idl' =>
+      match store_init_data m b p id cp with
+      | None => None
+      | Some m' => store_init_data_list m' b (p + init_data_size id) idl' cp
+      end
+  end.
+
+Definition perm_globvar (gv: globvar V) : permission :=
+  if gv.(gvar_volatile) then Nonempty
+  else if gv.(gvar_readonly) then Readable
+  else Writable.
+
+Definition alloc_global (m: mem) (idg: ident * globdef F V): option mem :=
+  match idg with
+  | (id, Gfun f) =>
+      let (m1, b) := Mem.alloc m (comp_of f) 0 1 in
+      Mem.drop_perm m1 b 0 1 Nonempty (comp_of f)
+  | (id, Gvar v) =>
+      let init := v.(gvar_init) in
+      let comp := v.(gvar_comp) in
+      let sz := init_data_list_size init in
+      let (m1, b) := Mem.alloc m comp 0 sz in
+      match store_zeros m1 b 0 sz comp with
+      | None => None
+      | Some m2 =>
+          match store_init_data_list m2 b 0 init comp with
+          | None => None
+          | Some m3 => Mem.drop_perm m3 b 0 sz (perm_globvar v) comp
+          end
+      end
+  end.
+
+Fixpoint alloc_globals (m: mem) (gl: list (ident * globdef F V))
+                       {struct gl} : option mem :=
+  match gl with
+  | nil => Some m
+  | g :: gl' =>
+      match alloc_global m g with
+      | None => None
+      | Some m' => alloc_globals m' gl'
+      end
+  end.
+
+Lemma alloc_globals_app : forall gl1 gl2 m m1,
+  alloc_globals m gl1 = Some m1 ->
+  alloc_globals m1 gl2 = alloc_globals m (gl1 ++ gl2).
+Proof.
+  induction gl1.
+  simpl. intros.  inversion H; subst. auto.
+  simpl. intros. destruct (alloc_global m a); eauto. inversion H.
+Qed.
+
+(** Next-block properties *)
+
+Remark store_zeros_nextblock:
+  forall m b p n cp m', store_zeros m b p n cp = Some m' -> Mem.nextblock m' = Mem.nextblock m.
+Proof.
+  intros until cp. functional induction (store_zeros m b p n cp); intros.
+  inv H; auto.
+  rewrite IHo; eauto with mem.
+  congruence.
+Qed.
+
+Remark store_init_data_list_nextblock:
+  forall idl b m p cp m',
+  store_init_data_list m b p idl cp = Some m' ->
+  Mem.nextblock m' = Mem.nextblock m.
+Proof.
+  induction idl; simpl; intros until m'.
+  intros. congruence.
+  caseEq (store_init_data m b p a cp); try congruence. intros.
+  transitivity (Mem.nextblock m0). eauto.
+  destruct a; simpl in H; try (eapply Mem.nextblock_store; eauto; fail).
+  congruence.
+  destruct (find_symbol ge i); try congruence. eapply Mem.nextblock_store; eauto.
+Qed.
+
+Remark alloc_global_nextblock:
+  forall g m m',
+  alloc_global m g = Some m' ->
+  Mem.nextblock m' = Pos.succ(Mem.nextblock m).
+Proof.
+  unfold alloc_global. intros.
+  destruct g as [id [f|v]].
+- (* function *)
+  destruct (Mem.alloc m _ 0 1) as [m1 b] eqn:?.
+  erewrite Mem.nextblock_drop; eauto.
+  now erewrite Mem.nextblock_alloc; eauto.
+- (* variable *)
+  set (init := gvar_init v) in *.
+  set (sz := init_data_list_size init) in *.
+  destruct (Mem.alloc m _ 0 sz) as [m1 b] eqn:?.
+  destruct (store_zeros m1 b 0 sz) as [m2|] eqn:?; try discriminate.
+  destruct (store_init_data_list m2 b 0 init) as [m3|] eqn:?; try discriminate.
+  erewrite Mem.nextblock_drop; eauto.
+  erewrite store_init_data_list_nextblock; eauto.
+  erewrite store_zeros_nextblock; eauto.
+  erewrite Mem.nextblock_alloc; eauto.
+Qed.
+
+Remark alloc_globals_nextblock:
+  forall gl m m',
+  alloc_globals m gl = Some m' ->
+  Mem.nextblock m' = advance_next gl (Mem.nextblock m).
+Proof.
+  induction gl; simpl; intros.
+  congruence.
+  destruct (alloc_global m a) as [m1|] eqn:?; try discriminate.
+  erewrite IHgl; eauto. erewrite alloc_global_nextblock; eauto.
+Qed.
+
+(** Block compartments *)
+
+Remark store_zeros_block_compartment:
+  forall m b p n cp m', store_zeros m b p n cp = Some m' ->
+  forall b', Mem.block_compartment m' b' = Mem.block_compartment m b'.
+Proof.
+  intros m b p n cp.
+  functional induction (store_zeros m b p n cp)
+    as [|m b p n cp ? ? m' STORE IH|]; try congruence.
+  intros m'' STOREZEROS b'.
+  rewrite (IH _ STOREZEROS).
+  erewrite Mem.store_block_compartment; eauto.
+Qed.
+
+Remark store_init_data_block_compartment:
+  forall m b p id cp m',
+  store_init_data m b p id cp = Some m' ->
+  forall b', Mem.block_compartment m' b' = Mem.block_compartment m b'.
+Proof.
+  intros m b p id cp m'.
+  destruct id as [?|?|?|?|?|?|?|id off]; simpl;
+  try apply Mem.store_block_compartment.
+  - congruence.
+  - destruct find_symbol; try congruence.
+    apply Mem.store_block_compartment.
+Qed.
+
+Remark store_init_data_list_block_compartment:
+  forall m b p idl cp m',
+  store_init_data_list m b p idl cp = Some m' ->
+  forall b', Mem.block_compartment m' b' = Mem.block_compartment m b'.
+Proof.
+  intros m b p idl cp. revert m p.
+  induction idl as [|id idl IH]; intros m p; simpl.
+  - congruence.
+  - intros m'.
+    destruct store_init_data as [m''|] eqn:INITDATA; try congruence.
+    intros INITDATALIST b'. rewrite (IH _ _ _ INITDATALIST).
+    eapply store_init_data_block_compartment; eauto.
+Qed.
+
+Remark alloc_global_block_compartment:
+  forall m idg m' b,
+  alloc_global m idg = Some m' ->
+  Mem.block_compartment m' b =
+  if eq_block b (Mem.nextblock m) then Some (comp_of idg#2)
+  else Mem.block_compartment m b.
+Proof.
+intros m [id [v|f]] m' b ALLOCGLOB; simpl in *.
+- destruct (Mem.alloc _ _ _ _) as [m'' b'] eqn:ALLOC.
+  erewrite Mem.drop_block_compartment; eauto.
+  erewrite Mem.alloc_block_compartment; eauto.
+  erewrite <- Mem.alloc_result; eauto.
+- destruct (Mem.alloc _ _ _ _) as [m0 b0] eqn:ALLOC.
+  destruct store_zeros as [m1|] eqn:STOREZEROS; try congruence.
+  destruct store_init_data_list as [m2|] eqn:INITDATALIST; try congruence.
+  erewrite Mem.drop_block_compartment; eauto.
+  erewrite store_init_data_list_block_compartment; eauto.
+  erewrite store_zeros_block_compartment; eauto.
+  erewrite Mem.alloc_block_compartment; eauto.
+  erewrite <- Mem.alloc_result; eauto.
+Qed.
+
+Fixpoint alloc_globals_block_compartment_spec
+         dflt b0 (gl : list (ident * globdef F V)) b : option block :=
+  match gl with
+  | nil => dflt
+  | g :: gl =>
+    let dflt' := if eq_block b b0 then Some (comp_of g#2)
+                 else dflt in
+    alloc_globals_block_compartment_spec dflt' (Pos.succ b0) gl b
+  end.
+
+Remark alloc_globals_block_compartment:
+  forall m gl m',
+  alloc_globals m gl = Some m' ->
+  forall b, Mem.block_compartment m' b =
+  alloc_globals_block_compartment_spec
+    (Mem.block_compartment m b) (Mem.nextblock m) gl b.
+Proof.
+intros m gl m' ALLOC b. revert m m' ALLOC.
+induction gl as [|g gl IH]; simpl; try congruence.
+intros m1 m3 ALLOCGLOBALS.
+destruct alloc_global as [m2|] eqn:ALLOC; try congruence.
+rewrite (IH _ _ ALLOCGLOBALS), (alloc_global_block_compartment _ _ _ ALLOC).
+erewrite <- alloc_global_nextblock; eauto.
+Qed.
+
+(** Permissions *)
+
+Remark store_zeros_perm:
+  forall k prm b' q m b p n cp m',
+  store_zeros m b p n cp = Some m' ->
+  (Mem.perm m b' q k prm <-> Mem.perm m' b' q k prm).
+Proof.
+  intros until cp. functional induction (store_zeros m b p n cp); intros.
+  inv H; tauto.
+  destruct (IHo _ H); intros. split; eauto with mem.
+  congruence.
+Qed.
+
+Remark store_init_data_perm:
+  forall k prm b' q i cp b m p m',
+  store_init_data m b p i cp = Some m' ->
+  (Mem.perm m b' q k prm <-> Mem.perm m' b' q k prm).
+Proof.
+  intros.
+  assert (forall chunk v,
+          Mem.store chunk m b p v cp = Some m' ->
+          (Mem.perm m b' q k prm <-> Mem.perm m' b' q k prm)).
+    intros; split; eauto with mem.
+  destruct i; simpl in H; eauto.
+  inv H; tauto.
+  destruct (find_symbol ge i); try discriminate. eauto.
+Qed.
+
+Remark store_init_data_list_perm:
+  forall k prm b' q idl cp b m p m',
+  store_init_data_list m b p idl cp = Some m' ->
+  (Mem.perm m b' q k prm <-> Mem.perm m' b' q k prm).
+Proof.
+  induction idl as [ | i1 idl]; simpl; intros.
+- inv H; tauto.
+- destruct (store_init_data m b p i1) as [m1|] eqn:S1; try discriminate.
+  transitivity (Mem.perm m1 b' q k prm).
+  eapply store_init_data_perm; eauto.
+  eapply IHidl; eauto.
+Qed.
+
+Remark alloc_global_perm:
+  forall k prm b' q idg m m',
+  alloc_global m idg = Some m' ->
+  Mem.valid_block m b' ->
+  (Mem.perm m b' q k prm <-> Mem.perm m' b' q k prm).
+Proof.
+  intros. destruct idg as [id [f|v]]; simpl in H.
+- (* function *)
+  destruct (Mem.alloc m _ 0 1) as [m1 b] eqn:?.
+  assert (b' <> b). apply Mem.valid_not_valid_diff with m; eauto with mem.
+  split; intros.
+  eapply Mem.perm_drop_3; eauto. eapply Mem.perm_alloc_1; eauto.
+  eapply Mem.perm_alloc_4; eauto. eapply Mem.perm_drop_4; eauto.
+- (* variable *)
+  set (init := gvar_init v) in *.
+  set (sz := init_data_list_size init) in *.
+  destruct (Mem.alloc m _ 0 sz) as [m1 b] eqn:?.
+  destruct (store_zeros m1 b 0 sz) as [m2|] eqn:?; try discriminate.
+  destruct (store_init_data_list m2 b 0 init) as [m3|] eqn:?; try discriminate.
+  assert (b' <> b). apply Mem.valid_not_valid_diff with m; eauto with mem.
+  split; intros.
+  eapply Mem.perm_drop_3; eauto.
+  erewrite <- store_init_data_list_perm; [idtac|eauto].
+  erewrite <- store_zeros_perm; [idtac|eauto].
+  eapply Mem.perm_alloc_1; eauto.
+  eapply Mem.perm_alloc_4; eauto.
+  erewrite store_zeros_perm; [idtac|eauto].
+  erewrite store_init_data_list_perm; [idtac|eauto].
+  eapply Mem.perm_drop_4; eauto.
+Qed.
+
+Remark alloc_globals_perm:
+  forall k prm b' q gl m m',
+  alloc_globals m gl = Some m' ->
+  Mem.valid_block m b' ->
+  (Mem.perm m b' q k prm <-> Mem.perm m' b' q k prm).
+Proof.
+  induction gl.
+  simpl; intros. inv H. tauto.
+  simpl; intros. destruct (alloc_global m a) as [m1|] eqn:?; try discriminate.
+  erewrite alloc_global_perm; eauto. eapply IHgl; eauto.
+  unfold Mem.valid_block in *. erewrite alloc_global_nextblock; eauto.
+  apply Plt_trans_succ; auto.
+Qed.
+
+(** Data preservation properties *)
+
+Remark store_zeros_unchanged:
+  forall (P: block -> Z -> Prop) m b p n cp m',
+  store_zeros m b p n cp = Some m' ->
+  (forall i, p <= i < p + n -> ~ P b i) ->
+  Mem.unchanged_on P m m'.
+Proof.
+  intros until cp. functional induction (store_zeros m b p n cp); intros.
+- inv H; apply Mem.unchanged_on_refl.
+- apply Mem.unchanged_on_trans with m'.
++ eapply Mem.store_unchanged_on; eauto. simpl. intros. apply H0. omega.
++ apply IHo; auto. intros; apply H0; omega.
+- discriminate.
+Qed.
+
+Remark store_init_data_unchanged:
+  forall (P: block -> Z -> Prop) b i cp m p m',
+  store_init_data m b p i cp = Some m' ->
+  (forall ofs, p <= ofs < p + init_data_size i -> ~ P b ofs) ->
+  Mem.unchanged_on P m m'.
+Proof.
+  intros. destruct i; simpl in *;
+  try (eapply Mem.store_unchanged_on; eauto; fail).
+  inv H; apply Mem.unchanged_on_refl.
+  destruct (find_symbol ge i); try congruence.
+  eapply Mem.store_unchanged_on; eauto;
+  unfold Mptr; destruct Archi.ptr64; eauto.
+Qed.
+
+Remark store_init_data_list_unchanged:
+  forall (P: block -> Z -> Prop) b il cp m p m',
+  store_init_data_list m b p il cp = Some m' ->
+  (forall ofs, p <= ofs -> ~ P b ofs) ->
+  Mem.unchanged_on P m m'.
+Proof.
+  induction il; simpl; intros.
+- inv H. apply Mem.unchanged_on_refl.
+- destruct (store_init_data m b p a) as [m1|] eqn:?; try congruence.
+  apply Mem.unchanged_on_trans with m1.
+  eapply store_init_data_unchanged; eauto. intros; apply H0; tauto.
+  eapply IHil; eauto. intros; apply H0. generalize (init_data_size_pos a); omega.
+Qed.
+
+(** Properties related to [loadbytes] *)
+
+Definition readbytes_as_zero (m: mem) (b: block) (ofs len: Z) (cp: option compartment) : Prop :=
+  forall p n,
+  ofs <= p -> p + Z.of_nat n <= ofs + len ->
+  Mem.loadbytes m b p (Z.of_nat n) cp = Some (list_repeat n (Byte Byte.zero)).
+
+Lemma store_zeros_loadbytes:
+  forall m b p n cp m',
+    Mem.can_access_block m b (Some cp) ->
+  store_zeros m b p n cp = Some m' ->
+  readbytes_as_zero m' b p n (Some cp) /\ Mem.can_access_block m' b (Some cp).
+Proof.
+  intros until cp.
+  functional induction (store_zeros m b p n cp).
+- split; [red|]; intros.
+  destruct n0. simpl. apply Mem.loadbytes_empty. omega.
+  inv H0; eauto.
+  rewrite Nat2Z.inj_succ in H2. omegaContradiction.
+  inv H0; eauto.
+- split; [red|]; intros.
+  destruct (zeq p0 p).
+  + subst p0. destruct n0. simpl. apply Mem.loadbytes_empty. omega.
+    eapply IHo in H0 as [? ?]; eauto.
+    eapply Mem.store_can_access_block_2; eauto.
+    rewrite Nat2Z.inj_succ in H2. rewrite Nat2Z.inj_succ.
+    replace (Z.succ (Z.of_nat n0)) with (1 + Z.of_nat n0) by omega.
+    change (list_repeat (S n0) (Byte Byte.zero))
+      with ((Byte Byte.zero :: nil) ++ list_repeat n0 (Byte Byte.zero)).
+    apply Mem.loadbytes_concat.
+    eapply Mem.loadbytes_unchanged_on with (P := fun b1 ofs1 => ofs1 = p).
+    eapply store_zeros_unchanged; eauto. intros; omega.
+    intros; omega.
+    replace (Byte Byte.zero :: nil) with (encode_val Mint8unsigned Vzero).
+    change 1 with (size_chunk Mint8unsigned).
+    eapply Mem.loadbytes_store_same; eauto.
+    unfold encode_val; unfold encode_int; unfold rev_if_be; destruct Archi.big_endian; reflexivity.
+    eapply IHo; eauto.
+    eapply Mem.store_can_access_block_2; eauto.
+    omega. omega. omega. omega.
+  + eapply IHo; eauto.
+    eapply Mem.store_can_access_block_2; eauto.
+    omega. omega.
+  + eapply IHo; eauto.
+    eapply Mem.store_can_access_block_2; eauto.
+- discriminate.
+Qed.
+
+Definition bytes_of_init_data (i: init_data): list memval :=
+  match i with
+  | Init_int8 n => inj_bytes (encode_int 1%nat (Int.unsigned n))
+  | Init_int16 n => inj_bytes (encode_int 2%nat (Int.unsigned n))
+  | Init_int32 n => inj_bytes (encode_int 4%nat (Int.unsigned n))
+  | Init_int64 n => inj_bytes (encode_int 8%nat (Int64.unsigned n))
+  | Init_float32 n => inj_bytes (encode_int 4%nat (Int.unsigned (Float32.to_bits n)))
+  | Init_float64 n => inj_bytes (encode_int 8%nat (Int64.unsigned (Float.to_bits n)))
+  | Init_space n => list_repeat (Z.to_nat n) (Byte Byte.zero)
+  | Init_addrof id ofs =>
+      match find_symbol ge id with
+      | Some b => inj_value (if Archi.ptr64 then Q64 else Q32) (Vptr b ofs)
+      | None   => list_repeat (if Archi.ptr64 then 8%nat else 4%nat) Undef
+      end
+  end.
+
+Remark init_data_size_addrof:
+  forall id ofs, init_data_size (Init_addrof id ofs) = size_chunk Mptr.
+Proof.
+  intros. unfold Mptr. simpl. destruct Archi.ptr64; auto.
+Qed.
+
+Lemma store_init_data_loadbytes:
+  forall m b p i cp m',
+  store_init_data m b p i cp = Some m' ->
+  readbytes_as_zero m b p (init_data_size i) (Some cp) ->
+  Mem.loadbytes m' b p (init_data_size i) (Some cp) = Some (bytes_of_init_data i).
+Proof.
+  intros; destruct i; simpl in H; try apply (Mem.loadbytes_store_same _ _ _ _ _ _ _ H).
+- inv H. simpl.
+  assert (EQ: Z.of_nat (Z.to_nat z) = Z.max z 0).
+  { destruct (zle 0 z). rewrite Z2Nat.id; xomega. destruct z; try discriminate. simpl. xomega. }
+  rewrite <- EQ. apply H0. omega. simpl. omega.
+- rewrite init_data_size_addrof. simpl.
+  destruct (find_symbol ge i) as [b'|]; try discriminate.
+  rewrite (Mem.loadbytes_store_same _ _ _ _ _ _ _ H).
+  unfold encode_val, Mptr; destruct Archi.ptr64; reflexivity.
+Qed.
+
+Fixpoint bytes_of_init_data_list (il: list init_data): list memval :=
+  match il with
+  | nil => nil
+  | i :: il => bytes_of_init_data i ++ bytes_of_init_data_list il
+  end.
+
+Lemma store_init_data_list_loadbytes:
+  forall b il m p cp m',
+    Mem.can_access_block m b (Some cp) ->
+  store_init_data_list m b p il cp = Some m' ->
+  readbytes_as_zero m b p (init_data_list_size il) (Some cp) ->
+  Mem.loadbytes m' b p (init_data_list_size il) (Some cp) = Some (bytes_of_init_data_list il).
+Proof.
+  induction il as [ | i1 il]; simpl; intros.
+- apply Mem.loadbytes_empty. omega. inv H0; eauto.
+- generalize (init_data_size_pos i1) (init_data_list_size_pos il); intros P1 PL.
+  destruct (store_init_data m b p i1) as [m1|] eqn:S; try discriminate.
+  apply Mem.loadbytes_concat.
+  eapply Mem.loadbytes_unchanged_on with (P := fun b1 ofs1 => ofs1 < p + init_data_size i1).
+  eapply store_init_data_list_unchanged; eauto.
+  intros; omega.
+  intros; omega.
+  eapply store_init_data_loadbytes; eauto.
+  red; intros; apply H1. omega. omega.
+  apply IHil with m1; auto.
+  unfold store_init_data in S; destruct i1; try now eapply Mem.store_can_access_block_2; eauto.
+  inv S; eauto. destruct (find_symbol ge i); try discriminate.
+  now eapply Mem.store_can_access_block_2; eauto.
+  red; intros.
+  eapply Mem.loadbytes_unchanged_on with (P := fun b1 ofs1 => p + init_data_size i1 <= ofs1).
+  eapply store_init_data_unchanged; eauto.
+  intros; omega.
+  intros; omega.
+  apply H1. omega. omega.
+  auto. auto.
+Qed.
+
+(** Properties related to [load] *)
+
+Definition read_as_zero (m: mem) (b: block) (ofs len: Z) (cp: option compartment) : Prop :=
+  forall chunk p,
+  ofs <= p -> p + size_chunk chunk <= ofs + len ->
+  (align_chunk chunk | p) ->
+  Mem.load chunk m b p cp =
+  Some (match chunk with
+        | Mint8unsigned | Mint8signed | Mint16unsigned | Mint16signed | Mint32 => Vint Int.zero
+        | Mint64 => Vlong Int64.zero
+        | Mfloat32 => Vsingle Float32.zero
+        | Mfloat64 => Vfloat Float.zero
+        | Many32 | Many64 => Vundef
+        end).
+
+Remark read_as_zero_unchanged:
+  forall (P: block -> Z -> Prop) m b ofs len cp m',
+  read_as_zero m b ofs len cp ->
+  Mem.unchanged_on P m m' ->
+  (forall i, ofs <= i < ofs + len -> P b i) ->
+  read_as_zero m' b ofs len cp.
+Proof.
+  intros; red; intros. eapply Mem.load_unchanged_on; eauto.
+  intros; apply H1. omega.
+Qed.
+
+Lemma store_zeros_read_as_zero:
+  forall m b p n cp m',
+    Mem.can_access_block m b (Some cp) ->
+  store_zeros m b p n cp = Some m' ->
+  read_as_zero m' b p n (Some cp).
+Proof.
+  intros; red; intros.
+  transitivity (Some(decode_val chunk (list_repeat (size_chunk_nat chunk) (Byte Byte.zero)))).
+  apply Mem.loadbytes_load; auto. rewrite size_chunk_conv.
+  eapply store_zeros_loadbytes; eauto. rewrite <- size_chunk_conv; auto.
+  f_equal. destruct chunk; unfold decode_val; unfold decode_int; unfold rev_if_be; destruct Archi.big_endian; reflexivity.
+Qed.
+
+Fixpoint load_store_init_data (m: mem) (b: block) (p: Z) (il: list init_data) (cp: option compartment) {struct il} : Prop :=
+  match il with
+  | nil => True
+  | Init_int8 n :: il' =>
+      Mem.load Mint8unsigned m b p cp = Some(Vint(Int.zero_ext 8 n))
+      /\ load_store_init_data m b (p + 1) il' cp
+  | Init_int16 n :: il' =>
+      Mem.load Mint16unsigned m b p cp = Some(Vint(Int.zero_ext 16 n))
+      /\ load_store_init_data m b (p + 2) il' cp
+  | Init_int32 n :: il' =>
+      Mem.load Mint32 m b p cp = Some(Vint n)
+      /\ load_store_init_data m b (p + 4) il' cp
+  | Init_int64 n :: il' =>
+      Mem.load Mint64 m b p cp = Some(Vlong n)
+      /\ load_store_init_data m b (p + 8) il' cp
+  | Init_float32 n :: il' =>
+      Mem.load Mfloat32 m b p cp = Some(Vsingle n)
+      /\ load_store_init_data m b (p + 4) il' cp
+  | Init_float64 n :: il' =>
+      Mem.load Mfloat64 m b p cp = Some(Vfloat n)
+      /\ load_store_init_data m b (p + 8) il' cp
+  | Init_addrof symb ofs :: il' =>
+      (exists b', find_symbol ge symb = Some b' /\ Mem.load Mptr m b p cp = Some(Vptr b' ofs))
+      /\ load_store_init_data m b (p + size_chunk Mptr) il' cp
+  | Init_space n :: il' =>
+      read_as_zero m b p n cp
+      /\ load_store_init_data m b (p + Z.max n 0) il' cp
+  end.
+
+Lemma store_init_data_list_charact:
+  forall b il m p cp m',
+  store_init_data_list m b p il cp = Some m' ->
+  read_as_zero m b p (init_data_list_size il) (Some cp) ->
+  load_store_init_data m' b p il (Some cp).
+Proof.
+  assert (A: forall chunk v m b p m1 il cp m',
+    Mem.store chunk m b p v cp = Some m1 ->
+    store_init_data_list m1 b (p + size_chunk chunk) il cp = Some m' ->
+    Mem.load chunk m' b p (Some cp) = Some(Val.load_result chunk v)).
+  {
+    intros.
+    eapply Mem.load_unchanged_on with (P := fun b' ofs' => ofs' < p + size_chunk chunk).
+    eapply store_init_data_list_unchanged; eauto. intros; omega.
+    intros; tauto.
+    eapply Mem.load_store_same; eauto.
+  }
+  induction il; simpl.
+- auto.
+- intros. destruct (store_init_data m b p a) as [m1|] eqn:?; try congruence.
+  exploit IHil; eauto.
+  set (P := fun (b': block) ofs' => p + init_data_size a <= ofs').
+  apply read_as_zero_unchanged with (m := m) (P := P).
+  red; intros; apply H0; auto. generalize (init_data_size_pos a); omega. omega.
+  eapply store_init_data_unchanged with (P := P); eauto.
+  intros; unfold P. omega.
+  intros; unfold P. omega.
+  intro D.
+  destruct a; simpl in Heqo.
++ split; auto. eapply (A Mint8unsigned (Vint i)); eauto.
++ split; auto. eapply (A Mint16unsigned (Vint i)); eauto.
++ split; auto. eapply (A Mint32 (Vint i)); eauto.
++ split; auto. eapply (A Mint64 (Vlong i)); eauto.
++ split; auto. eapply (A Mfloat32 (Vsingle f)); eauto.
++ split; auto. eapply (A Mfloat64 (Vfloat f)); eauto.
++ split; auto.
+  set (P := fun (b': block) ofs' => ofs' < p + init_data_size (Init_space z)).
+  inv Heqo. apply read_as_zero_unchanged with (m := m1) (P := P).
+  red; intros. apply H0; auto. simpl. generalize (init_data_list_size_pos il); xomega.
+  eapply store_init_data_list_unchanged; eauto.
+  intros; unfold P. omega.
+  intros; unfold P. simpl; xomega.
++ rewrite init_data_size_addrof in *.
+  split; auto.
+  destruct (find_symbol ge i); try congruence.
+  exists b0; split; auto.
+  transitivity (Some (Val.load_result Mptr (Vptr b0 i0))).
+  eapply (A Mptr (Vptr b0 i0)); eauto.
+  unfold Val.load_result, Mptr; destruct Archi.ptr64; auto.
+Qed.
+
+Remark alloc_global_unchanged:
+  forall (P: block -> Z -> Prop) m id g m',
+  alloc_global m (id, g) = Some m' ->
+  Mem.unchanged_on P m m'.
+Proof.
+  intros. destruct g as [f|v]; simpl in H.
+- (* function *)
+  destruct (Mem.alloc m _ 0 1) as [m1 b] eqn:?.
+  set (Q := fun b' (ofs: Z) => b' <> b).
+  apply Mem.unchanged_on_implies with Q.
+  apply Mem.unchanged_on_trans with m1.
+  eapply Mem.alloc_unchanged_on; eauto.
+  eapply Mem.drop_perm_unchanged_on; eauto.
+  intros; red. apply Mem.valid_not_valid_diff with m; eauto with mem.
+- (* variable *)
+  set (init := gvar_init v) in *.
+  set (sz := init_data_list_size init) in *.
+  destruct (Mem.alloc m _ 0 sz) as [m1 b] eqn:?.
+  destruct (store_zeros m1 b 0 sz) as [m2|] eqn:?; try discriminate.
+  destruct (store_init_data_list m2 b 0 init) as [m3|] eqn:?; try discriminate.
+  set (Q := fun b' (ofs: Z) => b' <> b).
+  apply Mem.unchanged_on_implies with Q.
+  apply Mem.unchanged_on_trans with m1.
+  eapply Mem.alloc_unchanged_on; eauto.
+  apply Mem.unchanged_on_trans with m2.
+  eapply store_zeros_unchanged; eauto.
+  apply Mem.unchanged_on_trans with m3.
+  eapply store_init_data_list_unchanged; eauto.
+  eapply Mem.drop_perm_unchanged_on; eauto.
+  intros; red. apply Mem.valid_not_valid_diff with m; eauto with mem.
+Qed.
+
+Remark alloc_globals_unchanged:
+  forall (P: block -> Z -> Prop) gl m m',
+  alloc_globals m gl = Some m' ->
+  Mem.unchanged_on P m m'.
+Proof.
+  induction gl; simpl; intros.
+- inv H. apply Mem.unchanged_on_refl.
+- destruct (alloc_global m a) as [m''|] eqn:?; try discriminate.
+  destruct a as [id g].
+  apply Mem.unchanged_on_trans with m''.
+  eapply alloc_global_unchanged; eauto.
+  apply IHgl; auto.
+Qed.
+
+Remark load_store_init_data_invariant:
+  forall m m' b,
+  (forall chunk ofs cp, Mem.load chunk m' b ofs cp = Mem.load chunk m b ofs cp) ->
+  forall il p cp,
+  load_store_init_data m b p il cp -> load_store_init_data m' b p il cp.
+Proof.
+  induction il; intro p; simpl.
+  auto.
+  intros. rewrite ! H. destruct a; intuition. red; intros; rewrite H; auto.
+Qed.
+
+Definition globals_initialized (g: t) (m: mem) :=
+  forall b gd,
+  find_def g b = Some gd ->
+  match gd with
+  | Gfun f =>
+    Mem.perm m b 0 Cur Nonempty
+      /\ (forall ofs k p, Mem.perm m b ofs k p -> ofs = 0 /\ p = Nonempty)
+  | Gvar v =>
+         Mem.range_perm m b 0 (init_data_list_size v.(gvar_init)) Cur (perm_globvar v)
+      /\ (forall ofs k p, Mem.perm m b ofs k p ->
+            0 <= ofs < init_data_list_size v.(gvar_init) /\ perm_order (perm_globvar v) p)
+      /\ (v.(gvar_volatile) = false -> load_store_init_data m b 0 v.(gvar_init) (Some v.(gvar_comp)))
+      /\ (v.(gvar_volatile) = false -> Mem.loadbytes m b 0 (init_data_list_size v.(gvar_init)) (Some v.(gvar_comp)) = Some (bytes_of_init_data_list v.(gvar_init)))
+  end.
+
+Lemma alloc_global_initialized:
+  forall g m id gd m',
+  genv_next g = Mem.nextblock m ->
+  alloc_global m (id, gd) = Some m' ->
+  globals_initialized g m ->
+     globals_initialized (add_global g (id, gd)) m'
+  /\ genv_next (add_global g (id, gd)) = Mem.nextblock m'.
+Proof.
+  intros.
+  exploit alloc_global_nextblock; eauto. intros NB. split.
+- (* globals-initialized *)
+  red; intros. unfold find_def in H2; simpl in H2.
+  rewrite PTree.gsspec in H2. destruct (peq b (genv_next g)).
++ inv H2. destruct gd0 as [f|v]; simpl in H0.
+* destruct (Mem.alloc m _ 0 1) as [m1 b] eqn:ALLOC.
+  exploit Mem.alloc_result; eauto. intros RES.
+  rewrite H, <- RES. split.
+  eapply Mem.perm_drop_1; eauto. omega.
+  intros.
+  assert (0 <= ofs < 1). { eapply Mem.perm_alloc_3; eauto. eapply Mem.perm_drop_4; eauto. }
+  exploit Mem.perm_drop_2; eauto. intros ORD.
+  split. omega. inv ORD; auto.
+* set (init := gvar_init v) in *.
+  set (sz := init_data_list_size init) in *.
+  destruct (Mem.alloc m _ 0 sz) as [m1 b] eqn:?.
+  destruct (store_zeros m1 b 0 sz) as [m2|] eqn:?; try discriminate.
+  destruct (store_init_data_list m2 b 0 init) as [m3|] eqn:?; try discriminate.
+  exploit Mem.alloc_result; eauto. intro RES.
+  replace (genv_next g) with b by congruence.
+  split. red; intros. eapply Mem.perm_drop_1; eauto.
+  split. intros.
+  assert (0 <= ofs < sz).
+  { eapply Mem.perm_alloc_3; eauto.
+    erewrite store_zeros_perm by eauto.
+    erewrite store_init_data_list_perm by eauto.
+    eapply Mem.perm_drop_4; eauto. }
+  split; auto.
+  eapply Mem.perm_drop_2; eauto.
+  split. intros NOTVOL. apply load_store_init_data_invariant with m3.
+  intros. eapply Mem.load_drop; eauto. right; right; right.
+  unfold perm_globvar. rewrite NOTVOL. destruct (gvar_readonly v); auto with mem.
+  eapply store_init_data_list_charact; eauto.
+  eapply store_zeros_read_as_zero; eauto. eapply Mem.owned_new_block; eauto.
+  intros NOTVOL.
+  transitivity (Mem.loadbytes m3 b 0 sz (Some v.(gvar_comp))).
+  eapply Mem.loadbytes_drop; eauto. right; right; right.
+  unfold perm_globvar. rewrite NOTVOL. destruct (gvar_readonly v); auto with mem.
+  eapply store_init_data_list_loadbytes; eauto.
+  eapply store_zeros_loadbytes; eauto. eapply Mem.owned_new_block; eauto.
+  eapply store_zeros_loadbytes; eauto. eapply Mem.owned_new_block; eauto.
++ assert (U: Mem.unchanged_on (fun _ _ => True) m m') by (eapply alloc_global_unchanged; eauto).
+  assert (VALID: Mem.valid_block m b).
+  { red. rewrite <- H. eapply genv_defs_range; eauto. }
+  exploit H1; eauto.
+  destruct gd0 as [f|v].
+* intros [A B]; split; intros.
+  eapply Mem.perm_unchanged_on; eauto. exact I.
+  eapply B. eapply Mem.perm_unchanged_on_2; eauto. exact I.
+* intros (A & B & C & D). split; [| split; [| split]].
+  red; intros. eapply Mem.perm_unchanged_on; eauto. exact I.
+  intros. eapply B. eapply Mem.perm_unchanged_on_2; eauto. exact I.
+  intros. apply load_store_init_data_invariant with m; auto.
+  intros. eapply Mem.load_unchanged_on_1; eauto. intros; exact I.
+  intros. eapply Mem.loadbytes_unchanged_on; eauto. intros; exact I.
+- simpl. congruence.
+Qed.
+
+Lemma alloc_globals_initialized:
+  forall gl ge m m',
+  alloc_globals m gl = Some m' ->
+  genv_next ge = Mem.nextblock m ->
+  globals_initialized ge m ->
+  globals_initialized (add_globals ge gl) m'.
+Proof.
+  induction gl; simpl; intros.
+- inv H; auto.
+- destruct a as [id g]. destruct (alloc_global m (id, g)) as [m1|] eqn:?; try discriminate.
+  exploit alloc_global_initialized; eauto. intros [P Q].
+  eapply IHgl; eauto.
+Qed.
+
+End INITMEM.
+
+Definition init_mem (p: program F V) :=
+  alloc_globals (globalenv p) Mem.empty p.(prog_defs).
+
+Lemma init_mem_find_def:
+  forall p m b g,
+  init_mem p = Some m ->
+  find_def (globalenv p) b = Some g ->
+  Mem.block_compartment m b = Some (comp_of g).
+Proof.
+  intros p m b g.
+  unfold init_mem, find_def.
+  intros ALLOC.
+  rewrite (alloc_globals_block_compartment _ _ _ ALLOC). clear ALLOC.
+  unfold globalenv.
+  assert (Mem.block_compartment Mem.empty b = None) as ->.
+  { rewrite <- Mem.block_compartment_valid_block.
+    unfold Mem.valid_block. rewrite Mem.nextblock_empty.
+    now destruct b. }
+  simpl.
+  set (ge := empty_genv _ _).
+  change 1%positive with (genv_next ge).
+  assert (forall g', (genv_defs ge) ! b = Some g' ->
+                     None = Some (comp_of g')) as INV.
+  { intros g'. unfold ge. simpl. now rewrite PTree.gempty. }
+  generalize ge (@None compartment) INV. clear ge INV.
+  generalize (prog_defs p). clear p. intros idgl.
+  induction idgl as [|idg idgl IH]; simpl.
+  - eauto.
+  - intros ge o INV. apply IH. clear IH g.
+    intros g. simpl. destruct eq_block as [->|neq].
+    + rewrite PTree.gss. intros H. now injection H as <-.
+    + rewrite PTree.gso; trivial. apply INV.
+Qed.
+
+Lemma init_mem_genv_next: forall p m,
+  init_mem p = Some m ->
+  genv_next (globalenv p) = Mem.nextblock m.
+Proof.
+  unfold init_mem; intros.
+  exploit alloc_globals_nextblock; eauto. rewrite Mem.nextblock_empty. intro.
+  generalize (genv_next_add_globals (prog_defs p) (empty_genv (prog_public p) (prog_pol p))).
+  fold (globalenv p). simpl genv_next. intros. congruence.
+Qed.
+
+Theorem find_symbol_not_fresh:
+  forall p id b m,
+  init_mem p = Some m ->
+  find_symbol (globalenv p) id = Some b -> Mem.valid_block m b.
+Proof.
+  intros. red. erewrite <- init_mem_genv_next; eauto.
+  eapply genv_symb_range; eauto.
+Qed.
+
+Theorem find_def_not_fresh:
+  forall p b g m,
+  init_mem p = Some m ->
+  find_def (globalenv p) b = Some g -> Mem.valid_block m b.
+Proof.
+  intros. red. erewrite <- init_mem_genv_next; eauto.
+  eapply genv_defs_range; eauto.
+Qed.
+
+Theorem find_funct_ptr_not_fresh:
+  forall p b f m,
+  init_mem p = Some m ->
+  find_funct_ptr (globalenv p) b = Some f -> Mem.valid_block m b.
+Proof.
+  intros. rewrite find_funct_ptr_iff in H0. eapply find_def_not_fresh; eauto.
+Qed.
+
+Theorem find_var_info_not_fresh:
+  forall p b gv m,
+  init_mem p = Some m ->
+  find_var_info (globalenv p) b = Some gv -> Mem.valid_block m b.
+Proof.
+  intros. rewrite find_var_info_iff in H0. eapply find_def_not_fresh; eauto.
+Qed.
+
+Lemma init_mem_characterization_gen:
+  forall p m,
+  init_mem p = Some m ->
+  globals_initialized (globalenv p) (globalenv p) m.
+Proof.
+  intros. apply alloc_globals_initialized with Mem.empty.
+  auto.
+  rewrite Mem.nextblock_empty. auto.
+  red; intros. unfold find_def in H0; simpl in H0; rewrite PTree.gempty in H0; discriminate.
+Qed.
+
+Theorem init_mem_characterization:
+  forall p b gv m,
+  find_var_info (globalenv p) b = Some gv ->
+  init_mem p = Some m ->
+  Mem.range_perm m b 0 (init_data_list_size gv.(gvar_init)) Cur (perm_globvar gv)
+  /\ (forall ofs k p, Mem.perm m b ofs k p ->
+        0 <= ofs < init_data_list_size gv.(gvar_init) /\ perm_order (perm_globvar gv) p)
+  /\ (gv.(gvar_volatile) = false ->
+      load_store_init_data (globalenv p) m b 0 gv.(gvar_init) (Some gv.(gvar_comp)))
+  /\ (gv.(gvar_volatile) = false ->
+      Mem.loadbytes m b 0 (init_data_list_size gv.(gvar_init)) (Some gv.(gvar_comp)) = Some (bytes_of_init_data_list (globalenv p) gv.(gvar_init))).
+Proof.
+  intros. rewrite find_var_info_iff in H.
+  exploit init_mem_characterization_gen; eauto.
+Qed.
+
+Theorem init_mem_characterization_2:
+  forall p b fd m,
+  find_funct_ptr (globalenv p) b = Some fd ->
+  init_mem p = Some m ->
+  Mem.perm m b 0 Cur Nonempty
+  /\ (forall ofs k p, Mem.perm m b ofs k p -> ofs = 0 /\ p = Nonempty).
+Proof.
+  intros. rewrite find_funct_ptr_iff in H.
+  exploit init_mem_characterization_gen; eauto.
+Qed.
+
+(** ** Compatibility with memory injections *)
+
+Section INITMEM_INJ.
+
+Variable ge: t.
+Variable thr: block.
+Hypothesis symb_inject: forall id b, find_symbol ge id = Some b -> Plt b thr.
+
+Lemma store_zeros_neutral:
+  forall m b p n cp m',
+  Mem.inject_neutral thr m ->
+  Plt b thr ->
+  store_zeros m b p n cp = Some m' ->
+  Mem.inject_neutral thr m'.
+Proof.
+  intros until cp. functional induction (store_zeros m b p n cp); intros.
+  inv H1; auto.
+  apply IHo; auto. eapply Mem.store_inject_neutral; eauto. constructor.
+  inv H1.
+Qed.
+
+Lemma store_init_data_neutral:
+  forall m b p id cp m',
+  Mem.inject_neutral thr m ->
+  Plt b thr ->
+  store_init_data ge m b p id cp = Some m' ->
+  Mem.inject_neutral thr m'.
+Proof.
+  intros.
+  destruct id; simpl in H1; try (eapply Mem.store_inject_neutral; eauto; fail).
+  congruence.
+  destruct (find_symbol ge i) as [b'|] eqn:E; try discriminate.
+  eapply Mem.store_inject_neutral; eauto.
+  econstructor. unfold Mem.flat_inj. apply pred_dec_true; auto. eauto.
+  rewrite Ptrofs.add_zero. auto.
+Qed.
+
+Lemma store_init_data_list_neutral:
+  forall b idl m p cp m',
+  Mem.inject_neutral thr m ->
+  Plt b thr ->
+  store_init_data_list ge m b p idl cp = Some m' ->
+  Mem.inject_neutral thr m'.
+Proof.
+  induction idl; simpl; intros.
+  congruence.
+  destruct (store_init_data ge m b p a) as [m1|] eqn:E; try discriminate.
+  eapply IHidl. eapply store_init_data_neutral; eauto. auto. eauto.
+Qed.
+
+Lemma alloc_global_neutral:
+  forall idg m m',
+  alloc_global ge m idg = Some m' ->
+  Mem.inject_neutral thr m ->
+  Plt (Mem.nextblock m) thr ->
+  Mem.inject_neutral thr m'.
+Proof.
+  intros. destruct idg as [id [f|v]]; simpl in H.
+- (* function *)
+  destruct (Mem.alloc m _ 0 1) as [m1 b] eqn:?.
+  assert (Plt b thr). rewrite (Mem.alloc_result _ _ _ _ _ _ Heqp). auto.
+  eapply Mem.drop_inject_neutral; eauto.
+  eapply Mem.alloc_inject_neutral; eauto.
+- (* variable *)
+  set (init := gvar_init v) in *.
+  set (sz := init_data_list_size init) in *.
+  destruct (Mem.alloc m _ 0 sz) as [m1 b] eqn:?.
+  destruct (store_zeros m1 b 0 sz) as [m2|] eqn:?; try discriminate.
+  destruct (store_init_data_list ge m2 b 0 init) as [m3|] eqn:?; try discriminate.
+  assert (Plt b thr). rewrite (Mem.alloc_result _ _ _ _ _ _ Heqp). auto.
+  eapply Mem.drop_inject_neutral; eauto.
+  eapply store_init_data_list_neutral with (m := m2) (b := b); eauto.
+  eapply store_zeros_neutral with (m := m1); eauto.
+  eapply Mem.alloc_inject_neutral; eauto.
+Qed.
+
+Remark advance_next_le: forall gl x, Ple x (advance_next gl x).
+Proof.
+  induction gl; simpl; intros.
+  apply Ple_refl.
+  apply Ple_trans with (Pos.succ x). apply Ple_succ. eauto.
+Qed.
+
+Lemma alloc_globals_neutral:
+  forall gl m m',
+  alloc_globals ge m gl = Some m' ->
+  Mem.inject_neutral thr m ->
+  Ple (Mem.nextblock m') thr ->
+  Mem.inject_neutral thr m'.
+Proof.
+  induction gl; intros.
+  simpl in *. congruence.
+  exploit alloc_globals_nextblock; eauto. intros EQ.
+  simpl in *. destruct (alloc_global ge m a) as [m1|] eqn:E; try discriminate.
+  exploit alloc_global_neutral; eauto.
+  assert (Ple (Pos.succ (Mem.nextblock m)) (Mem.nextblock m')).
+  { rewrite EQ. apply advance_next_le. }
+  unfold Plt, Ple in *; zify; omega.
+Qed.
+
+End INITMEM_INJ.
+
+Theorem initmem_inject:
+  forall p m,
+  init_mem p = Some m ->
+  Mem.inject (Mem.flat_inj (Mem.nextblock m)) m m.
+Proof.
+  unfold init_mem; intros.
+  apply Mem.neutral_inject.
+  eapply alloc_globals_neutral; eauto.
+  intros. exploit find_symbol_not_fresh; eauto.
+  apply Mem.empty_inject_neutral.
+  apply Ple_refl.
+Qed.
+
+(** ** Sufficient and necessary conditions for the initial memory to exist. *)
+
+(** Alignment properties *)
+
+Definition init_data_alignment (i: init_data) : Z :=
+  match i with
+  | Init_int8 n => 1
+  | Init_int16 n => 2
+  | Init_int32 n => 4
+  | Init_int64 n => 8
+  | Init_float32 n => 4
+  | Init_float64 n => 4
+  | Init_addrof symb ofs => if Archi.ptr64 then 8 else 4
+  | Init_space n => 1
+  end.
+
+Fixpoint init_data_list_aligned (p: Z) (il: list init_data) {struct il} : Prop :=
+  match il with
+  | nil => True
+  | i1 :: il => (init_data_alignment i1 | p) /\ init_data_list_aligned (p + init_data_size i1) il
+  end.
+
+Section INITMEM_INVERSION.
+
+Variable ge: t.
+
+Lemma store_init_data_aligned:
+  forall m b p i cp m',
+  store_init_data ge m b p i cp = Some m' ->
+  (init_data_alignment i | p).
+Proof.
+  intros.
+  assert (DFL: forall chunk v,
+    Mem.store chunk m b p v cp = Some m' ->
+    align_chunk chunk = init_data_alignment i ->
+    (init_data_alignment i | p)).
+  { intros. apply Mem.store_valid_access_3 in H0. destruct H0 as [? [? ?]]. congruence. }
+  destruct i; simpl in H; eauto.
+  simpl. apply Z.divide_1_l.
+  destruct (find_symbol ge i); try discriminate. eapply DFL. eassumption.
+  unfold Mptr, init_data_alignment; destruct Archi.ptr64; auto.
+Qed.
+
+Lemma store_init_data_list_aligned:
+  forall b il m p cp m',
+  store_init_data_list ge m b p il cp = Some m' ->
+  init_data_list_aligned p il.
+Proof.
+  induction il as [ | i1 il]; simpl; intros.
+- auto.
+- destruct (store_init_data ge m b p i1) as [m1|] eqn:S1; try discriminate.
+  split; eauto. eapply store_init_data_aligned; eauto.
+Qed.
+
+Lemma store_init_data_list_free_idents:
+  forall b i o il m p cp m',
+  store_init_data_list ge m b p il cp = Some m' ->
+  In (Init_addrof i o) il ->
+  exists b', find_symbol ge i = Some b'.
+Proof.
+  induction il as [ | i1 il]; simpl; intros.
+- contradiction.
+- destruct (store_init_data ge m b p i1) as [m1|] eqn:S1; try discriminate.
+  destruct H0.
++ subst i1. simpl in S1. destruct (find_symbol ge i) as [b'|]. exists b'; auto. discriminate.
++ eapply IHil; eauto.
+Qed.
+
+End INITMEM_INVERSION.
+
+Theorem init_mem_inversion:
+  forall p m id v,
+  init_mem p = Some m ->
+  In (id, Gvar v) p.(prog_defs) ->
+  init_data_list_aligned 0 v.(gvar_init)
+  /\ forall i o, In (Init_addrof i o) v.(gvar_init) -> exists b, find_symbol (globalenv p) i = Some b.
+Proof.
+  intros until v. unfold init_mem. set (ge := globalenv p).
+  revert m. generalize Mem.empty. generalize (prog_defs p).
+  induction l as [ | idg1 defs ]; simpl; intros m m'; intros.
+- contradiction.
+- destruct (alloc_global ge m idg1) as [m''|] eqn:A; try discriminate.
+  destruct H0.
++ subst idg1; simpl in A.
+  set (il := gvar_init v) in *. set (sz := init_data_list_size il) in *.
+  destruct (Mem.alloc m _ 0 sz) as [m1 b].
+  destruct (store_zeros m1 b 0 sz) as [m2|]; try discriminate.
+  destruct (store_init_data_list ge m2 b 0 il) as [m3|] eqn:B; try discriminate.
+  split. eapply store_init_data_list_aligned; eauto. intros; eapply store_init_data_list_free_idents; eauto.
++ eapply IHdefs; eauto.
+Qed.
+
+Section INITMEM_EXISTS.
+
+Variable ge: t.
+
+Lemma store_zeros_exists:
+  forall m b p n cp,
+    Mem.range_perm m b p (p + n) Cur Writable ->
+    Mem.can_access_block m b (Some cp) ->
+  exists m', store_zeros m b p n cp = Some m'.
+Proof.
+  intros until cp. functional induction (store_zeros m b p n cp); intros PERM ACC.
+- exists m; auto.
+- intros. apply IHo. red; intros. eapply Mem.perm_store_1; eauto. apply PERM. omega.
+  eapply (Mem.store_can_access_block_inj _ _ _ _ _ _ _ e0). eauto.
+- destruct (Mem.valid_access_store m Mint8unsigned b p cp Vzero) as (m' & STORE).
+  split. red; intros. apply Mem.perm_cur. apply PERM. simpl in H. omega.
+  split. auto.
+  simpl. apply Z.divide_1_l.
+  congruence.
+Qed.
+
+Lemma store_init_data_exists:
+  forall m b p i cp,
+  Mem.range_perm m b p (p + init_data_size i) Cur Writable ->
+  forall OWN : Mem.can_access_block m b (Some cp),
+  (init_data_alignment i | p) ->
+  (forall id ofs, i = Init_addrof id ofs -> exists b, find_symbol ge id = Some b) ->
+  exists m', store_init_data ge m b p i cp = Some m'.
+Proof.
+  intros.
+  assert (DFL: forall chunk v,
+          init_data_size i = size_chunk chunk ->
+          init_data_alignment i = align_chunk chunk ->
+          exists m', Mem.store chunk m b p v cp = Some m').
+  { intros. destruct (Mem.valid_access_store m chunk b p cp v) as (m' & STORE).
+    split. rewrite <- H2; auto. rewrite <- H3; auto.
+    exists m'; auto. }
+  destruct i; eauto.
+  simpl. exists m; auto.
+  simpl. exploit H1; eauto. intros (b1 & FS). rewrite FS. eapply DFL.
+  unfold init_data_size, Mptr. destruct Archi.ptr64; auto.
+  unfold init_data_alignment, Mptr. destruct Archi.ptr64; auto.
+Qed.
+
+Lemma store_init_data_list_exists:
+  forall b il m p cp,
+  Mem.range_perm m b p (p + init_data_list_size il) Cur Writable ->
+  forall OWN : Mem.can_access_block m b (Some cp),
+  init_data_list_aligned p il ->
+  (forall id ofs, In (Init_addrof id ofs) il -> exists b, find_symbol ge id = Some b) ->
+  exists m', store_init_data_list ge m b p il cp = Some m'.
+Proof.
+  induction il as [ | i1 il ]; simpl; intros.
+- exists m; auto.
+- destruct H0.
+  destruct (@store_init_data_exists m b p i1 cp) as (m1 & S1); eauto.
+  red; intros. apply H. generalize (init_data_list_size_pos il); omega.
+  rewrite S1.
+  apply IHil; eauto.
+  red; intros. erewrite <- store_init_data_perm by eauto. apply H. generalize (init_data_size_pos i1); omega.
+
+  destruct i1; inv S1;
+    try eapply (Mem.store_can_access_block_inj _ _ _ _ _ _ _ H4); eauto.
+  destruct (find_symbol ge i); try discriminate.
+  eapply (Mem.store_can_access_block_inj _ _ _ _ _ _ _ H4). eauto.
+Qed.
+
+
+Lemma alloc_global_exists:
+  forall m idg,
+  match idg with
+  | (id, Gfun f) => True
+  | (id, Gvar v) =>
+        init_data_list_aligned 0 v.(gvar_init)
+     /\ forall i o, In (Init_addrof i o) v.(gvar_init) -> exists b, find_symbol ge i = Some b
+  end ->
+  exists m', alloc_global ge m idg = Some m'.
+Proof.
+  intros m [id [f|v]]; intros; simpl.
+- destruct (Mem.alloc m _ 0 1) as [m1 b] eqn:ALLOC.
+  destruct (Mem.range_perm_drop_2 m1 b 0 1 (comp_of f) Nonempty) as [m2 DROP].
+  red; intros; eapply Mem.perm_alloc_2; eauto.
+  eapply Mem.owned_new_block; eauto.
+  exists m2; auto.
+- destruct H as [P Q].
+  set (sz := init_data_list_size (gvar_init v)).
+  destruct (Mem.alloc m _ 0 sz) as [m1 b] eqn:ALLOC.
+  assert (P1: Mem.range_perm m1 b 0 sz Cur Freeable) by (red; intros; eapply Mem.perm_alloc_2; eauto).
+  destruct (@store_zeros_exists m1 b 0 sz (gvar_comp v)) as [m2 ZEROS].
+  red; intros. apply Mem.perm_implies with Freeable; auto with mem.
+  eapply Mem.owned_new_block; eauto.
+  rewrite ZEROS.
+  assert (P2: Mem.range_perm m2 b 0 sz Cur Freeable).
+  { red; intros. erewrite <- store_zeros_perm by eauto. eauto. }
+  destruct (@store_init_data_list_exists b (gvar_init v) m2 0 (gvar_comp v)) as [m3 STORE]; auto.
+  red; intros. apply Mem.perm_implies with Freeable; auto with mem.
+  eapply store_zeros_block_compartment with (b' := b) in ZEROS.
+  unfold Mem.can_access_block.  rewrite ZEROS. eapply Mem.owned_new_block. eauto.
+  rewrite STORE.
+  assert (P3: Mem.range_perm m3 b 0 sz Cur Freeable).
+  { red; intros. erewrite <- store_init_data_list_perm by eauto. eauto. }
+  destruct (Mem.range_perm_drop_2 m3 b 0 sz (gvar_comp v) (perm_globvar v)) as [m4 DROP]; auto.
+  eapply store_init_data_list_block_compartment with (b' := b) in STORE.
+  eapply store_zeros_block_compartment with (b' := b) in ZEROS.
+  unfold Mem.can_access_block.  rewrite STORE, ZEROS. eapply Mem.owned_new_block. eauto.
+  exists m4; auto.
+Qed.
+
+End INITMEM_EXISTS.
+
+Theorem init_mem_exists:
+  forall p,
+  (forall id v, In (id, Gvar v) (prog_defs p) ->
+        init_data_list_aligned 0 v.(gvar_init)
+     /\ forall i o, In (Init_addrof i o) v.(gvar_init) -> exists b, find_symbol (globalenv p) i = Some b) ->
+  exists m, init_mem p = Some m.
+Proof.
+  intros. set (ge := globalenv p) in *.
+  unfold init_mem. revert H. generalize (prog_defs p) Mem.empty.
+  induction l as [ | idg l]; simpl; intros.
+- exists m; auto.
+- destruct (@alloc_global_exists ge m idg) as [m1 A1].
+  destruct idg as [id [f|v]]; eauto.
+  fold ge. rewrite A1. eapply IHl; eauto.
+Qed.
+
+(* Allowed cross-compartment calls *)
+Definition allowed_cross_call (ge: t) (cp: compartment) (vf: val) :=
+  match vf with
+  | Vptr b _ =>
+    exists i cp',
+    invert_symbol ge b = Some i /\
+    find_comp ge vf = cp' /\
+    match (Policy.policy_import ge.(genv_policy)) ! cp with
+    | Some l => In (cp', i) l
+    | None => False
+    end /\
+    match (Policy.policy_export ge.(genv_policy)) ! cp' with
+    | Some l => In i l
+    | None => False
+    end
+  | _ => False
+  end.
+
+Variant call_type :=
+  | InternalCall
+  | CrossCompartmentCall
+  | DefaultCompartmentCall
+.
+
+Definition type_of_call (ge: t) (cp: compartment) (cp': compartment): call_type :=
+  if Pos.eqb cp cp' then InternalCall
+  else if Pos.eqb cp' default_compartment then DefaultCompartmentCall
+       else CrossCompartmentCall.
+
+(* Definition type_of_call (ge: t) (cp: compartment) (vf: val): call_type := *)
+(*   match find_comp ge vf with *)
+(*   | None => InternalCall (* a failed call is internal, by definition *) *)
+(*   | Some cp' => type_of_call ge cp cp' *)
+(*       (* if Pos.eqb cp cp' then InternalCall *) *)
+(*       (* else if Pos.eqb cp' default_compartment then DefaultCompartmentCall *) *)
+(*       (*      else CrossCompartmentCall *) *)
+(*   end. *)
+
+(* (* A call is cross-compartment if the following definition holds: *) *)
+(* Definition cross_call (ge: t) (cp: compartment) (vf: val) := *)
+(*   match find_comp ge vf with *)
+(*   | Some cp' => cp <> cp' /\ *)
+(*                  cp' <> default_compartment (* the default compartment is really privileged, *)
+(*                                             as this is where all the builtin functions live *) *)
+(*   | None => False *)
+(*   end. *)
+
+(* Definition cross_call_b (ge: t) (cp: compartment) (vf: val): bool := *)
+(*   match find_comp ge vf with *)
+(*   | Some cp' => negb (Pos.eqb cp cp') && negb (Pos.eqb cp' default_compartment) *)
+(*   | None => false *)
+(*   end. *)
+
+(* Lemma cross_call_reflect: forall ge cp vf, *)
+(*     cross_call ge cp vf <-> cross_call_b ge cp vf = true. *)
+(* Proof. *)
+(*   intros. *)
+(*   unfold cross_call, cross_call_b. *)
+(*   destruct (find_comp ge vf) eqn:COMP. *)
+(*   - split. *)
+(*     + intros [cp_neq cp_neq']. *)
+(*       apply Pos.eqb_neq in cp_neq. apply Pos.eqb_neq in cp_neq'. *)
+(*       rewrite cp_neq, cp_neq'. reflexivity. *)
+(*     + intros cp_neq. apply andb_true_iff in cp_neq as [cp_neq cp_neq']. *)
+(*       apply negb_true_iff in cp_neq. apply negb_true_iff in cp_neq'. *)
+(*       split; apply Pos.eqb_neq; assumption. *)
+(*   - split; [auto | discriminate]. *)
+(* Qed. *)
+
+(* A call is allowed if any of these 3 cases holds:
+(1) the procedure being called belongs to the default compartment
+(2) the procedure being called belongs to the same compartment as the caller
+(3) the call is an inter-compartment call and is allowed by the policy
+*)
+Definition allowed_call (ge: t) (cp: compartment) (vf: val) :=
+  default_compartment = find_comp ge vf \/ (* TODO: does this mean we allow all compartment to perform IO calls? *)
+  cp = find_comp ge vf \/
+  allowed_cross_call ge cp vf.
+
+Lemma comp_ident_eq_dec: forall (x y: compartment * ident),
+    {x = y} + {x <> y}.
+Proof.
+  intros x y.
+  decide equality.
+  eapply Pos.eq_dec.
+  eapply Pos.eq_dec.
+Qed.
+
+Definition allowed_call_b (ge: t) (cp: compartment) (vf: val): bool :=
+  match find_comp ge vf with
+  | c => Pos.eqb c default_compartment
+             || Pos.eqb c cp
+             || match vf with
+               | Vptr b _ => match invert_symbol ge b with
+                            | Some i =>
+                              match (Policy.policy_import ge.(genv_policy)) ! cp with
+                              | Some imps =>
+                                match (Policy.policy_export ge.(genv_policy)) ! c with
+                                | Some exps =>
+                                  in_dec comp_ident_eq_dec (c, i) imps &&
+                                  in_dec Pos.eq_dec i exps
+                                | None => false
+                                end
+                              | None => false
+                              end
+                            | None => false
+                            end
+               | _ => false
+               end
+  end.
+
+Lemma allowed_call_reflect: forall ge cp vf,
+    allowed_call ge cp vf <-> allowed_call_b ge cp vf = true.
+Proof.
+  intros ge cp vf.
+  unfold allowed_call, allowed_call_b, allowed_cross_call.
+  destruct vf eqn:VF; try (firstorder; discriminate).
+  (* destruct (find_comp ge (Vptr b i)) eqn:COMP; try (firstorder; discriminate). *)
+  remember (find_comp ge (Vptr b i)) as c.
+  destruct (Pos.eq_dec default_compartment c); subst.
+  - rewrite <- e. split; auto.
+  - destruct (Pos.eq_dec (find_comp ge (Vptr b i)) cp); subst.
+    (* destruct (Pos.eq_dec c cp); subst. *)
+    + rewrite Pos.eqb_refl. rewrite orb_true_r. simpl. split; auto.
+    + split; auto.
+      * intros H. destruct H as [? | [? | ?]]; try congruence.
+        destruct H as [i' [cp' [H1 [H2 [H3 H4]]]]].
+        rewrite H1. inv H2.
+        destruct ((Policy.policy_import (genv_policy ge)) ! cp) as [imps |]; auto.
+        destruct ((Policy.policy_export (genv_policy ge)) ! (find_comp ge (Vptr b i))) as [exps |]; auto.
+        destruct (in_dec comp_ident_eq_dec ((find_comp ge (Vptr b i)), i') imps);
+          destruct (in_dec Pos.eq_dec i' exps); simpl; auto.
+        now rewrite orb_true_r.
+      * intros H.
+        right; right.
+        destruct (find_comp ge (Vptr b i)); try (now unfold default_compartment in n).
+        -- simpl in H. apply Pos.eqb_neq in n0. rewrite n0 in H. simpl in H.
+           destruct (invert_symbol ge b); try discriminate.
+           exists i0. exists (c~1)%positive. split; auto. split; auto. simpl.
+           destruct ((Policy.policy_import (genv_policy ge)) ! cp) as [imps |]; try discriminate.
+           destruct (Policy.policy_export (genv_policy ge)); try discriminate.
+           destruct (t0_2 ! c); try discriminate.
+           apply andb_prop in H.
+           destruct H as [H1 H2].
+           apply proj_sumbool_true in H1.
+           apply proj_sumbool_true in H2.
+           auto.
+        -- simpl in H. apply Pos.eqb_neq in n0. rewrite n0 in H. simpl in H.
+           destruct (invert_symbol ge b); try discriminate.
+           exists i0. exists (c~0)%positive. split; auto. split; auto. simpl.
+           destruct ((Policy.policy_import (genv_policy ge)) ! cp) as [imps |]; try discriminate.
+           destruct (Policy.policy_export (genv_policy ge)); try discriminate.
+           destruct (t0_1 ! c); try discriminate.
+           apply andb_prop in H.
+           destruct H as [H1 H2].
+           apply proj_sumbool_true in H1.
+           apply proj_sumbool_true in H2.
+           auto.
+Qed.
+
+End GENV.
+
+(** * Commutation with program transformations *)
+
+Section MATCH_GENVS.
+
+Context {A B V W: Type} (R: globdef A V -> globdef B W -> Prop).
+
+Record match_genvs (ge1: t A V) (ge2: t B W): Prop := {
+  mge_next:
+    genv_next ge2 = genv_next ge1;
+  mge_symb:
+    forall id, PTree.get id (genv_symb ge2) = PTree.get id (genv_symb ge1);
+  mge_defs:
+    forall b, option_rel R (PTree.get b (genv_defs ge1)) (PTree.get b (genv_defs ge2))
+}.
+
+Lemma add_global_match:
+  forall ge1 ge2 id g1 g2,
+  match_genvs ge1 ge2 ->
+  R g1 g2 ->
+  match_genvs (add_global ge1 (id, g1)) (add_global ge2 (id, g2)).
+Proof.
+  intros. destruct H. constructor; simpl; intros.
+- congruence.
+- rewrite mge_next0, ! PTree.gsspec. destruct (peq id0 id); auto.
+- rewrite mge_next0, ! PTree.gsspec. destruct (peq b (genv_next ge1)).
+  constructor; auto.
+  auto.
+Qed.
+
+Lemma add_globals_match:
+  forall gl1 gl2,
+  list_forall2 (fun idg1 idg2 => fst idg1 = fst idg2 /\ R (snd idg1) (snd idg2)) gl1 gl2 ->
+  forall ge1 ge2, match_genvs ge1 ge2 ->
+  match_genvs (add_globals ge1 gl1) (add_globals ge2 gl2).
+Proof.
+  induction 1; intros; simpl.
+  auto.
+  destruct a1 as [id1 g1]; destruct b1 as [id2 g2]; simpl in *; destruct H; subst id2.
+  apply IHlist_forall2. apply add_global_match; auto.
+Qed.
+
+End MATCH_GENVS.
+
+Section MATCH_PROGRAMS.
+
+Context {C F1 V1 F2 V2: Type} {LC: Linker C} {LF: Linker F1} {LV: Linker V1}.
+Context {CF1: has_comp F1} {CF2: has_comp F2}.
+Variable match_fundef: C -> F1 -> F2 -> Prop.
+Variable match_varinfo: V1 -> V2 -> Prop.
+Variable ctx: C.
+Variable p: program F1 V1.
+Variable tp: program F2 V2.
+Context {match_fundef_comp: has_comp_match match_fundef}.
+Hypothesis progmatch: match_program_gen match_fundef match_varinfo ctx p tp.
+
+Lemma globalenvs_match:
+  match_genvs (match_globdef match_fundef match_varinfo ctx) (globalenv p) (globalenv tp).
+Proof.
+  intros. apply add_globals_match. apply progmatch.
+  constructor; simpl; intros; auto. rewrite ! PTree.gempty. constructor.
+Qed.
+
+Theorem find_def_match_2:
+  forall b, option_rel (match_globdef match_fundef match_varinfo ctx)
+                       (find_def (globalenv p) b) (find_def (globalenv tp) b).
+Proof (mge_defs globalenvs_match).
+
+Theorem find_def_match:
+  forall b g,
+  find_def (globalenv p) b = Some g ->
+  exists tg,
+  find_def (globalenv tp) b = Some tg /\ match_globdef match_fundef match_varinfo ctx g tg.
+Proof.
+  intros. generalize (find_def_match_2 b). rewrite H; intros R; inv R.
+  exists y; auto.
+Qed.
+
+Theorem find_def_match_conv:
+  forall b tg,
+  find_def (globalenv tp) b = Some tg ->
+  exists g,
+  find_def (globalenv p) b = Some g /\ match_globdef match_fundef match_varinfo ctx g tg.
+Proof.
+  intros. generalize (find_def_match_2 b). rewrite H; intros R; inv R.
+  exists x; auto.
+Qed.
+
+Theorem find_funct_ptr_match:
+  forall b f,
+  find_funct_ptr (globalenv p) b = Some f ->
+  exists cunit tf,
+  find_funct_ptr (globalenv tp) b = Some tf /\ match_fundef cunit f tf /\ linkorder cunit ctx.
+Proof.
+  intros. rewrite find_funct_ptr_iff in *. apply find_def_match in H.
+  destruct H as (tg & P & Q). inv Q.
+  exists ctx', f2; intuition auto. apply find_funct_ptr_iff; auto.
+Qed.
+
+Theorem find_funct_ptr_match_conv:
+  forall b tf,
+  find_funct_ptr (globalenv tp) b = Some tf ->
+  exists cunit f,
+  find_funct_ptr (globalenv p) b = Some f /\ match_fundef cunit f tf /\ linkorder cunit ctx.
+Proof.
+  intros. rewrite find_funct_ptr_iff in *. apply find_def_match_conv in H.
+  destruct H as (tg & P & Q). inv Q.
+  exists ctx', f1; intuition auto. apply find_funct_ptr_iff; auto.
+Qed.
+
+Theorem find_funct_match:
+  forall v f,
+  find_funct (globalenv p) v = Some f ->
+  exists cunit tf,
+  find_funct (globalenv tp) v = Some tf /\ match_fundef cunit f tf /\ linkorder cunit ctx.
+Proof.
+  intros. exploit find_funct_inv; eauto. intros [b EQ]. subst v.
+  rewrite find_funct_find_funct_ptr in H.
+  rewrite find_funct_find_funct_ptr.
+  apply find_funct_ptr_match. auto.
+Qed.
+
+Theorem find_var_info_match:
+  forall b v,
+  find_var_info (globalenv p) b = Some v ->
+  exists tv,
+  find_var_info (globalenv tp) b = Some tv /\ match_globvar match_varinfo v tv.
+Proof.
+  intros. rewrite find_var_info_iff in *. apply find_def_match in H.
+  destruct H as (tg & P & Q). inv Q.
+  exists v2; split; auto. apply find_var_info_iff; auto.
+Qed.
+
+Theorem find_symbol_match:
+  forall (s : ident),
+  find_symbol (globalenv tp) s = find_symbol (globalenv p) s.
+Proof.
+  intros. destruct globalenvs_match. apply mge_symb0.
+Qed.
+
+Theorem senv_match:
+  Senv.equiv (to_senv (globalenv p)) (to_senv (globalenv tp)).
+Proof.
+  red; simpl. repeat split.
+- apply find_symbol_match.
+- intros. unfold public_symbol. rewrite find_symbol_match.
+  rewrite ! globalenv_public.
+  destruct progmatch as (P & Q & R & S). rewrite R. auto.
+- intros. unfold block_is_volatile.
+  destruct globalenvs_match as [P Q R]. specialize (R b).
+  unfold find_var_info, find_def.
+  inv R; auto.
+  inv H1; auto.
+  inv H2; auto.
+Qed.
+
+Lemma store_init_data_list_match:
+  forall idl m b ofs cp m',
+  store_init_data_list (globalenv p) m b ofs idl cp = Some m' ->
+  store_init_data_list (globalenv tp) m b ofs idl cp = Some m'.
+Proof.
+  induction idl; simpl; intros.
+- auto.
+- destruct (store_init_data (globalenv p) m b ofs a) as [m1|] eqn:S; try discriminate.
+  assert (X: store_init_data (globalenv tp) m b ofs a cp = Some m1).
+  { destruct a; auto. simpl; rewrite find_symbol_match; auto. }
+  rewrite X. auto.
+Qed.
+
+Lemma alloc_globals_match:
+  forall gl1 gl2, list_forall2 (match_ident_globdef match_fundef match_varinfo ctx) gl1 gl2 ->
+  forall m m',
+  alloc_globals (globalenv p) m gl1 = Some m' ->
+  alloc_globals (globalenv tp) m gl2 = Some m'.
+Proof.
+  induction 1; simpl; intros.
+- auto.
+- destruct (alloc_global (globalenv p) m a1) as [m1|] eqn:?; try discriminate.
+  assert (X: alloc_global (globalenv tp) m b1 = Some m1).
+  { destruct a1 as [id1 g1]; destruct b1 as [id2 g2]; destruct H; simpl in *.
+    subst id2. inv H2.
+  - erewrite <- match_fundef_comp; eauto.
+    erewrite <- match_fundef_comp; eauto.
+  - inv H; simpl in *. simpl in Heqo.
+    set (sz := init_data_list_size init) in *.
+    destruct (Mem.alloc m _ 0 sz) as [m2 b] eqn:?.
+    destruct (store_zeros m2 b 0 sz) as [m3|] eqn:?; try discriminate.
+    destruct (store_init_data_list (globalenv p) m3 b 0 init) as [m4|] eqn:?; try discriminate.
+    erewrite store_init_data_list_match; eauto.
+  }
+  rewrite X; eauto.
+Qed.
+
+Theorem init_mem_match:
+  forall m, init_mem p = Some m -> init_mem tp = Some m.
+Proof.
+  unfold init_mem; intros.
+  eapply alloc_globals_match; eauto. apply progmatch.
+Qed.
+
+Lemma match_genvs_find_comp:
+  forall vf,
+    find_comp (globalenv p) vf = find_comp (globalenv tp) vf.
+Proof.
+  intros vf.
+  unfold find_comp.
+  destruct vf; auto.
+  destruct (find_funct_ptr (globalenv p) b) eqn:EQ.
+  - apply find_funct_ptr_match in EQ as [? [? [H [? ?]]]]. rewrite H.
+    rewrite match_fundef_comp; eauto.
+  - destruct (find_funct_ptr (globalenv tp) b) eqn:EQ'.
+    + apply find_funct_ptr_match_conv in EQ' as [? [? [H [? ?]]]]. congruence.
+    + reflexivity.
+Qed.
+
+Lemma match_genvs_allowed_calls:
+  forall cp vf,
+    allowed_call (globalenv p) cp vf ->
+    allowed_call (globalenv tp) cp vf.
+Proof.
+  intros cp vf.
+  unfold allowed_call.
+  intros [H1 | [H1 | H1]].
+  - left. rewrite H1.
+    unfold find_comp in *. destruct vf; auto.
+    destruct (find_funct_ptr (globalenv p) b) eqn:EQ; auto.
+    apply find_funct_ptr_match in EQ as [? [? [? [? ?]]]].
+    rewrite H.
+    erewrite match_fundef_comp; eauto.
+    destruct (find_funct_ptr (globalenv tp) b) eqn:EQ'; auto.
+    apply find_funct_ptr_match_conv in EQ' as [? [? [? [? ?]]]].
+    congruence.
+  - right; left. rewrite H1.
+    unfold find_comp. destruct vf; auto.
+    destruct (find_funct_ptr (globalenv p) b) eqn:EQ; auto.
+    apply find_funct_ptr_match in EQ as [? [? [? [? ?]]]].
+    rewrite H.
+    erewrite match_fundef_comp; eauto.
+    destruct (find_funct_ptr (globalenv tp) b) eqn:EQ'; auto.
+    apply find_funct_ptr_match_conv in EQ' as [? [? [? [? ?]]]].
+    congruence.
+  - right; right.
+    unfold allowed_cross_call in *. destruct vf; eauto.
+    destruct H1 as [i0 [cp' [? [? [? ?]]]]].
+    exists i0; exists cp'; split; [| split; [| split]].
+    + apply find_invert_symbol. apply invert_find_symbol in H.
+      rewrite find_symbol_match; eauto.
+    + unfold find_comp in H0. unfold find_comp.
+      destruct (find_funct_ptr (globalenv p) b) eqn:EQ; auto.
+      apply find_funct_ptr_match in EQ as [? [? [? [? ?]]]].
+      rewrite H3.
+      inversion H0; subst.
+      rewrite match_fundef_comp. eauto. eauto.
+      destruct (find_funct_ptr (globalenv tp) b) eqn:EQ'; auto.
+      apply find_funct_ptr_match_conv in EQ' as [? [? [? [? ?]]]].
+      congruence.
+    + destruct progmatch as [? [? [? EQPOL]]].
+      destruct p, tp; simpl in *; subst.
+      unfold globalenv. unfold globalenv in H1.
+      simpl.
+      simpl in H1. clear -H1 EQPOL.
+
+      rewrite genv_pol_add_globals.
+      rewrite genv_pol_add_globals in H1.
+      unfold Policy.eqb in EQPOL. apply andb_prop in EQPOL.
+      destruct EQPOL as [EQPOL1 EQPOL2].
+      simpl in *.
+      rewrite PTree.beq_correct in EQPOL2. specialize (EQPOL2 cp).
+      destruct ((Policy.policy_import prog_pol0) ! cp);
+        destruct ((Policy.policy_import prog_pol) ! cp); auto.
+      destruct (Policy.list_cpt_id_eq l l0); subst; simpl in *; auto; try discriminate. contradiction.
+    + destruct progmatch as [? [? [? EQPOL]]].
+      destruct p, tp; simpl in *; subst.
+      unfold globalenv. unfold globalenv in H2.
+      simpl.
+      simpl in H2. clear -H2 EQPOL.
+
+      rewrite genv_pol_add_globals.
+      rewrite genv_pol_add_globals in H2.
+      unfold Policy.eqb in EQPOL. apply andb_prop in EQPOL.
+      destruct EQPOL as [EQPOL1 EQPOL2].
+      simpl in *.
+      rewrite PTree.beq_correct in EQPOL1.
+      remember (match find_funct_ptr (add_globals (empty_genv F1 V1 prog_public prog_pol) prog_defs) b with
+      | Some f => comp_of f
+      | None => default_compartment
+      end) as cp'.
+      (* destruct (find_funct_ptr (add_globals (empty_genv F1 V1 prog_public prog_pol) prog_defs) b) *)
+      specialize (EQPOL1 cp').
+      destruct ((Policy.policy_export prog_pol0) ! cp');
+        destruct ((Policy.policy_export prog_pol) ! cp'); subst cp'; auto; try contradiction.
+      destruct (Policy.list_id_eq l l0); subst; simpl in *; auto; try discriminate.
+Qed.
+
+Lemma match_genvs_type_of_call:
+  forall cp cp',
+    type_of_call (globalenv p) cp cp' (* (find_comp (globalenv p) vf) *) =
+      type_of_call (globalenv tp) cp cp' (* (find_comp (globalenv tp) vf) *).
+Proof.
+  intros. reflexivity.
+Qed.
+
+End MATCH_PROGRAMS.
+
+(** Special case for partial transformations that do not depend on the compilation unit *)
+
+Section TRANSFORM_PARTIAL.
+
+Context {A B V: Type} {LA: Linker A} {LV: Linker V}.
+Context {CA: has_comp A} {CB: has_comp B}.
+Context {transf: A -> res B} {p: program A V} {tp: program B V}.
+Context {CAB: has_comp_transl_partial transf}.
+Hypothesis progmatch: match_program (fun cu f tf => transf f = OK tf) eq p tp.
+
+Theorem find_funct_ptr_transf_partial:
+  forall b f,
+  find_funct_ptr (globalenv p) b = Some f ->
+  exists tf,
+  find_funct_ptr (globalenv tp) b = Some tf /\ transf f = OK tf.
+Proof.
+  intros. exploit (find_funct_ptr_match progmatch); eauto.
+  intros (cu & tf & P & Q & R); exists tf; auto.
+Qed.
+
+Theorem find_funct_ptr_transf_partial_conv:
+  forall b tf,
+  find_funct_ptr (globalenv tp) b = Some tf ->
+  exists f,
+  find_funct_ptr (globalenv p) b = Some f /\ transf f = OK tf.
+Proof.
+  intros. exploit (find_funct_ptr_match_conv progmatch); eauto.
+  intros (cu & f & P & Q & R); exists f; auto.
+Qed.
+
+Lemma find_comp_transf_partial:
+  forall v,
+  find_comp (globalenv p) v = find_comp (globalenv tp) v.
+Proof.
+  unfold find_comp. intros v.
+  destruct v as [| | | | |b ofs]; trivial.
+  destruct (find_funct_ptr (globalenv p) b) as [f|] eqn:Ef; try easy.
+  (* intros Ecp. *)
+  destruct (find_funct_ptr_transf_partial _ Ef) as (tf & H1 & H2).
+  now rewrite H1, <- (comp_transl_partial _ H2).
+  destruct (find_funct_ptr (globalenv tp) b) eqn:Etf; auto.
+  destruct (find_funct_ptr_transf_partial_conv _ Etf) as (f & H1 & H2).
+  congruence.
+Qed.
+
+Theorem find_funct_transf_partial:
+  forall v f,
+  find_funct (globalenv p) v = Some f ->
+  exists tf,
+  find_funct (globalenv tp) v = Some tf /\ transf f = OK tf.
+Proof.
+  intros. exploit (find_funct_match progmatch); eauto.
+  intros (cu & tf & P & Q & R); exists tf; auto.
+Qed.
+
+Theorem find_symbol_transf_partial:
+  forall (s : ident),
+  find_symbol (globalenv tp) s = find_symbol (globalenv p) s.
+Proof.
+  intros. eapply (find_symbol_match progmatch).
+Qed.
+
+Theorem senv_transf_partial:
+  Senv.equiv (to_senv (globalenv p)) (to_senv (globalenv tp)).
+Proof.
+  intros. eapply (senv_match progmatch).
+Qed.
+
+Theorem init_mem_transf_partial:
+  forall m, init_mem p = Some m -> init_mem tp = Some m.
+Proof.
+  eapply (init_mem_match progmatch).
+Qed.
+
+Theorem allowed_call_transf_partial:
+  forall cp vf,
+    allowed_call (globalenv p) cp vf -> allowed_call (globalenv tp) cp vf.
+Proof.
+  eapply (match_genvs_allowed_calls progmatch).
+Qed.
+
+Theorem type_of_call_transf_partial:
+  forall cp cp',
+    type_of_call (globalenv p) cp cp' =
+      type_of_call (globalenv tp) cp cp'.
+Proof.
+  eapply (match_genvs_type_of_call).
+Qed.
+
+End TRANSFORM_PARTIAL.
+
+(** Special case for total transformations that do not depend on the compilation unit *)
+
+Section TRANSFORM_TOTAL.
+
+Context {A B V: Type} {LA: Linker A} {LV: Linker V}.
+Context {CA: has_comp A} {CB: has_comp B}.
+Context {transf: A -> B} {p: program A V} {tp: program B V}.
+Context {CAB: has_comp_transl transf}.
+Hypothesis progmatch: match_program (fun cu f tf => tf = transf f) eq p tp.
+
+Theorem find_funct_ptr_transf:
+  forall b f,
+  find_funct_ptr (globalenv p) b = Some f ->
+  find_funct_ptr (globalenv tp) b = Some (transf f).
+Proof.
+  intros. exploit (find_funct_ptr_match progmatch); eauto.
+  intros (cu & tf & P & Q & R). congruence.
+Qed.
+
+Theorem find_funct_transf:
+  forall v f,
+  find_funct (globalenv p) v = Some f ->
+  find_funct (globalenv tp) v = Some (transf f).
+Proof.
+  intros. exploit (find_funct_match progmatch); eauto.
+  intros (cu & tf & P & Q & R). congruence.
+Qed.
+
+Theorem find_symbol_transf:
+  forall (s : ident),
+  find_symbol (globalenv tp) s = find_symbol (globalenv p) s.
+Proof.
+  intros. eapply (find_symbol_match progmatch).
+Qed.
+
+Theorem senv_transf:
+  Senv.equiv (to_senv (globalenv p)) (to_senv (globalenv tp)).
+Proof.
+  intros. eapply (senv_match progmatch).
+Qed.
+
+Theorem init_mem_transf:
+  forall m, init_mem p = Some m -> init_mem tp = Some m.
+Proof.
+  eapply (init_mem_match progmatch).
+Qed.
+
+Theorem allowed_call_transf:
+  forall cp vf,
+    allowed_call (globalenv p) cp vf -> allowed_call (globalenv tp) cp vf.
+Proof.
+  eapply (match_genvs_allowed_calls progmatch).
+Qed.
+
+Lemma find_comp_transf:
+  forall v,
+  find_comp (globalenv p) v = find_comp (globalenv tp) v.
+Proof.
+  unfold find_comp. intros v.
+  destruct v as [| | | | |b ofs]; trivial.
+  destruct (find_funct_ptr (globalenv p) b) as [f|] eqn:Ef; try easy.
+  (* intros Ecp. *)
+  rewrite (find_funct_ptr_transf _ Ef).
+  now rewrite comp_transl.
+  destruct (find_funct_ptr (globalenv tp) b) eqn:Etf; auto.
+  eapply (find_funct_ptr_match_conv progmatch) in Etf as [? [? [? [? ?]]]].
+  congruence.
+Qed.
+
+Theorem type_of_call_transf:
+  forall cp cp',
+    type_of_call (globalenv p) cp cp' =
+      type_of_call (globalenv tp) cp cp'.
+Proof.
+  eapply (match_genvs_type_of_call).
+Qed.
+
+End TRANSFORM_TOTAL.
+
+End Genv.
+
+Coercion Genv.to_senv: Genv.t >-> Senv.t.
